@prefix rdf:    <http://www.w3.org/1999/02/22-rdf-syntax-ns#> .
@prefix rdfs:   <http://www.w3.org/2000/01/rdf-schema#> .
@prefix owl:    <http://www.w3.org/2002/07/owl#> .
@prefix cc:     <http://creativecommons.org/ns#> .
@prefix xsd:    <http://www.w3.org/2001/XMLSchema#> .
@prefix dct:    <http://purl.org/dc/terms/> .
@prefix vann:   <http://purl.org/vocab/vann/> .
@prefix foaf:   <http://xmlns.com/foaf/0.1/> .
@prefix geo:    <https://www.w3.org/2003/01/geo/wgs84_pos#> .
@prefix osm:    <https://w3id.org/openstreetmap/terms#> .
@prefix qudt:   <http://qudt.org/schema/qudt/> .
@prefix unit:   <http://qudt.org/vocab/unit/> .
@prefix prov:   <http://www.w3.org/ns/prov#> .


# About

<https://w3id.org/openstreetmap/terms>
        a                 foaf:Document ;
        foaf:primaryTopic osm: .

osm:    a                              owl:Ontology ;
        dct:description                "This ontology describes the OpenStreetMap data model."@en ;
        cc:license                     <https://creativecommons.org/licenses/by/4.0/> ;
        rdfs:label                     "OpenStreetMaps Vocabulary"@en ;
        vann:preferredNamespacePrefix  "osm" ;
        vann:preferredNamespaceUri     "https://w3id.org/openstreetmap/terms#";
        dct:creator                    <https://biblio.ugent.be/person/802002413821> .

<https://biblio.ugent.be/person/802002413821> 
        a                 foaf:Person ;
        foaf:name         "Harm Delva" ;
        foaf:mbox         "harm.delva@ugent.be" .


# Element Classes

osm:Node  
        a                     rdfs:Class , owl:Class ;
        rdfs:comment          """A node is one of the core elements in the OpenStreetMap data model.
                              It consists of a single point in space defined by its latitude, longitude and node id."""@en ;
        rdfs:label            "Node"@en ;
        rdfs:subClassOf       geo:Point ;
        owl:disjointWith      osm:Way , osm:Relation ;
        rdfs:isDefinedBy      osm: ;
        prov:wasInfluencedBy  <https://wiki.openstreetmap.org/wiki/Node> .
        
osm:Way  
        a                     rdfs:Class , owl:Class ;
        rdfs:comment          "A way is an ordered list of nodes which normally also has at least one tag."@en ;
        rdfs:label            "Way"@en ;
        owl:disjointWith      osm:Node , osm:Relation ;
        rdfs:isDefinedBy      osm: ;
        prov:wasInfluencedBy  <https://wiki.openstreetmap.org/wiki/Way> .
        
osm:Relation  
        a                     rdfs:Class , owl:Class ;
        rdfs:comment          """A relation consists of one or more tags and also an ordered list of one or more nodes, ways and/or relations as members.
                              It is used to define logical or geographic relationships between other elements."""@en ;
        rdfs:label            "Relation"@en ;
        owl:disjointWith      osm:Node , osm:Way ;
        rdfs:isDefinedBy      osm: ;
        prov:wasInfluencedBy  <https://wiki.openstreetmap.org/wiki/Relation> .
        
osm:Element
        a                     rdfs:Class , owl:Class ;
        rdfs:comment          "Elements are the basic components of OpenStreetMap's conceptual data model of the physical world."@en ;
        rdfs:label            "Element"@en ;
        owl:unionOf           (osm:Node osm:Way osm:Relation) ;
        rdfs:isDefinedBy      osm: ;
        prov:wasInfluencedBy  <https://wiki.openstreetmap.org/wiki/Elements> .


# Object Properties

osm:hasNodes
        a                     owl:ObjectProperty , rdf:Property ;
        rdfs:comment          """An ordered collection of nodes that describe the way. 
                              These may be fragmented over multiple predicates due to tiling for example.
                              Each fragment should have enough overlap to reconstruct the original way."""@en ;
        rdfs:label            "hasNodes"@en ;
        rdfs:isDefinedBy      osm: ;
        rdfs:domain           osm:Way ;
        rdfs:range            rdf:list .

osm:access
        a                      owl:ObjectProperty , rdf:Property ;
        rdfs:comment           "Used to describe the legal access for highways and other transportation networks."@en ;
        rdfs:label             "access=*"@en ;
        rdfs:isDefinedBy       osm: ;
        prov:wasInfluencedBy   <https://wiki.openstreetmap.org/wiki/Key:access> ;
        rdfs:domain            osm:Element ;
        rdfs:range             osm:AccessValue .

osm:barrier
        a                      owl:ObjectProperty , rdf:Property ;
        owl:equivalentProperty <http://www.wikidata.org/entity/Q264661> ;
        rdfs:comment           "A barrier is a physical structure which blocks or impedes movement."@en ;
        rdfs:label             "barrier=*"@en ;
        rdfs:isDefinedBy       osm: ;
        prov:wasInfluencedBy   <https://wiki.openstreetmap.org/wiki/Key:barrier> ;
        rdfs:domain            osm:Element ;
        rdfs:range             osm:BarrierValue .

osm:bicycle
        a                      owl:ObjectProperty , rdf:Property ;
        rdfs:comment           "Legal restrictions for bicycles."@en ;
        rdfs:label             "bicycle=*"@en ;
        rdfs:isDefinedBy       osm: ;
        prov:wasInfluencedBy   <https://wiki.openstreetmap.org/wiki/Key:bicycle> ;
        rdfs:domain            osm:Element ;
        rdfs:range             osm:AccessValue .

osm:construction
        a                      owl:ObjectProperty , rdf:Property ;
        rdfs:comment           "Used to describe a feature which is currently under construction."@en ;
        rdfs:label             "construction=*"@en ;
        rdfs:isDefinedBy       osm: ;
        prov:wasInfluencedBy   <https://wiki.openstreetmap.org/wiki/Key:construction> ;
        rdfs:domain            osm:Element ;
        rdfs:range             osm:ConstructionValue .

osm:crossing
        a                      owl:ObjectProperty , rdf:Property ;
        rdfs:comment           "This tag is used for more accurately describing specific types of pedestrian crossings."@en ;
        rdfs:label             "crossing=*"@en ;
        rdfs:isDefinedBy       osm: ;
        prov:wasInfluencedBy   <https://wiki.openstreetmap.org/wiki/Key:crossing> ;
        rdfs:domain            osm:Element ;
        rdfs:range             osm:CrossingValue .

osm:cycleway
        a                      owl:ObjectProperty , rdf:Property ;
        rdfs:comment           "Maps cycling infrastructure that is an inherent part of the road."@en ;
        rdfs:label             "cycleway=*"@en ;
        rdfs:isDefinedBy       osm: ;
        prov:wasInfluencedBy   <https://wiki.openstreetmap.org/wiki/Key:cycleway> ;
        rdfs:domain            osm:Way ;
        rdfs:range             osm:CyclewayValue .

osm:footway
        a                      owl:ObjectProperty , rdf:Property ;
        rdfs:comment           "Refines the osm:Footway for sidewalks."@en ;
        rdfs:label             "footway=*"@en ;
        rdfs:isDefinedBy       osm: ;
        prov:wasInfluencedBy   <https://wiki.openstreetmap.org/wiki/Key:footway> ;
        rdfs:domain            osm:Way ;
        rdfs:range             osm:FootwayValue .

osm:highway
        a                      owl:ObjectProperty , rdf:Property ;
        owl:equivalentProperty <http://www.wikidata.org/entity/Q57977870> ;
        rdfs:comment           "This the main property used to identify any kind of road, street or path."@en ;
        rdfs:label             "highway=*"@en ;
        rdfs:isDefinedBy       osm: ;
        prov:wasInfluencedBy   <https://wiki.openstreetmap.org/wiki/Key:highway> ;
        rdfs:domain            osm:Element ;
        rdfs:range             osm:HighwayValue .

osm:motor_vehicle
        a                      owl:ObjectProperty , rdf:Property ;
        rdfs:comment           "Legal access restriction for all motor vehicles."@en ;
        rdfs:label             "motor_vehicle=*"@en ;
        rdfs:isDefinedBy       osm: ;
        prov:wasInfluencedBy   <https://wiki.openstreetmap.org/wiki/Key:motor_vehicle> ;
        rdfs:domain            osm:Way ;
        rdfs:range             osm:AccessValue .

osm:motorcar
        a                      owl:ObjectProperty , rdf:Property ;
        rdfs:comment           "Legal access permission for cars."@en ;
        rdfs:label             "motorcar=*"@en ;
        rdfs:isDefinedBy       osm: ;
        prov:wasInfluencedBy   <https://wiki.openstreetmap.org/wiki/Key:motorcar> ;
        rdfs:domain            osm:Way ;
        rdfs:range             osm:AccessValue .

osm:motorroad
        a                      owl:ObjectProperty , rdf:Property ;
        rdfs:comment           "Describe highways that have motorway-like access restrictions but that are not motorways."@en ;
        rdfs:label             "motorroad=*"@en ;
        rdfs:isDefinedBy       osm: ;
        prov:wasInfluencedBy   <https://wiki.openstreetmap.org/wiki/Key:motorroad> ;
        rdfs:domain            osm:Way ;
        rdfs:range             osm:MotorroadValue .

osm:mtb_scale
        a                      owl:ObjectProperty , rdf:Property ;
        rdfs:comment           "Provides a classification scheme for mapping the difficulty of trails suitable for mountain-biking."@en ;
        rdfs:label             "mtb:scale=*"@en ;
        rdfs:isDefinedBy       osm: ;
        prov:wasInfluencedBy   <https://wiki.openstreetmap.org/wiki/Key:mtb:scale> ;
        rdfs:domain            osm:Element ;
        rdfs:range             osm:MtbScaleValue .

osm:oneway_bicycle
        a                      owl:ObjectProperty , rdf:Property ;
        rdfs:comment           "Defines the oneway rules for cyclists."@en ;
        rdfs:label             "oneway:bicycle=*"@en ;
        rdfs:isDefinedBy       osm: ;
        prov:wasInfluencedBy   <https://wiki.openstreetmap.org/wiki/Key:oneway:bicycle> ;
        rdfs:domain            osm:Way ;
        rdfs:range             osm:OnewayValue .

osm:oneway
        a                      owl:ObjectProperty , rdf:Property ;
        owl:equivalentProperty <http://www.wikidata.org/entity/Q786886> ;
        rdfs:comment           "Indicate the access restriction on highways and other linear features."@en ;
        rdfs:label             "oneway=*"@en ;
        rdfs:isDefinedBy       osm: ;
        prov:wasInfluencedBy   <https://wiki.openstreetmap.org/wiki/Key:oneway> ;
        rdfs:domain            osm:Way ;
        rdfs:range             osm:OnewayValue .

osm:segregated
        a                      owl:ObjectProperty , rdf:Property ;
        rdfs:comment           "Used for combined cycle- and footways."@en ;
        rdfs:label             "segregated=*"@en ;
        rdfs:isDefinedBy       osm: ;
        prov:wasInfluencedBy   <https://wiki.openstreetmap.org/wiki/Key:segregated> ;
        rdfs:domain            osm:Way ;
        rdfs:range             osm:SegregatedValue .

osm:smoothness
        a                      owl:ObjectProperty , rdf:Property ;
        rdfs:comment           "Provides a classification scheme regarding the physical usability of a way."@en ;
        rdfs:label             "smoothness=*"@en ;
        rdfs:isDefinedBy       osm: ;
        prov:wasInfluencedBy   <hhttps://wiki.openstreetmap.org/wiki/Key:smoothness> ;
        rdfs:domain            osm:Way ;
        rdfs:range             osm:SmoothnessValue .

osm:surface
        a                      owl:ObjectProperty , rdf:Property ;
        owl:equivalentProperty <http://www.wikidata.org/entity/Q1049667> ;
        rdfs:comment           "Provides information about the physical surface of elements, particularly regarding material composition and/or structure."@en ;
        rdfs:label             "surface=*"@en ;
        rdfs:isDefinedBy       osm: ;
        prov:wasInfluencedBy   <https://wiki.openstreetmap.org/wiki/Key:surface> ;
        rdfs:domain            osm:Element ;
        rdfs:range             osm:SurfaceValue .

osm:tracktype
        a                      owl:ObjectProperty , rdf:Property ;
        rdfs:comment           "Measures how well-maintained a track is, particularly regarding surface firmness."@en ;
        rdfs:label             "tracktype=*"@en ;
        rdfs:isDefinedBy       osm: ;
        prov:wasInfluencedBy   <https://wiki.openstreetmap.org/wiki/Key:tracktype> ;
        rdfs:domain            osm:Way ;
        rdfs:range             osm:TracktypeValue .

osm:vehicle
        a                      owl:ObjectProperty , rdf:Property ;
        rdfs:comment           "Legal access restriction for all types of land-based vehicles not operated upon rails."@en ;
        rdfs:label             "vehicle=*"@en ;
        rdfs:isDefinedBy       osm: ;
        prov:wasInfluencedBy   <https://wiki.openstreetmap.org/wiki/Key:vehicle> ;
        rdfs:domain            osm:Way ;
        rdfs:range             osm:AccessValue .

# Data properties

osm:name
        a                       owl:DatatypeProperty , rdf:Property ;
        rdfs:subPropertyOf      dct:title ;
        owl:equivalentProperty  <http://www.wikidata.org/entity/Q82799> ;
        rdfs:comment            "Used for naming an element."@en ;
        rdfs:label              "name=*"@en ;
        rdfs:isDefinedBy        osm: ;
        prov:wasInfluencedBy    <https://wiki.openstreetmap.org/wiki/Key:name> ;
        rdfs:domain             osm:Element ;
        rdfs:range              rdfs:Literal .

osm:hasTag
        a                     owl:DatatypeProperty , rdf:Property ;
        rdfs:comment          """A tag describes the meaning of a particular element in the OSM data model. 
                              It consists of two free format text fields; a 'key' and a 'value' and are formatted as '{key}={value}'. 
                              This property should be used for tags that don't have their semantics explicitly defined. """@en ;
        rdfs:label            "hasTag"@en ;
        rdfs:isDefinedBy      osm: ;
        rdfs:domain           osm:Element ;
        rdfs:range            xsd:string .

osm:maxspeed
        a                     owl:DatatypeProperty , rdf:Property ;
        rdfs:comment          "Used to define the maximum legal speed limit, in km/h."@en ;
        rdfs:label            "maxspeed=*"@en ;
        rdfs:isDefinedBy      osm: ;
        prov:wasInfluencedBy  <https://wiki.openstreetmap.org/wiki/Key:maxspeed> ;
        qudt:hasUnit          unit:KM-PER-HR ;
        rdfs:domain           osm:Way ;
        rdfs:range            xsd:double .


# Tag Values

osm:AccessValue
        a                     rdfs:Class , owl:Class ;
        rdfs:comment          "Used to describe the legal access for highways and other transportation networks."@en ;
        rdfs:label            "AccessValue"@en ;
        rdfs:isDefinedBy      osm: ;
        prov:wasInfluencedBy  <https://wiki.openstreetmap.org/wiki/Key:access> .

osm:BarrierValue
        a                     rdfs:Class , owl:Class ;
        rdfs:comment          "A barrier is a physical structure which blocks or impedes movement."@en ;
        rdfs:label            "BarrierValue"@en ;
        rdfs:isDefinedBy      osm: ;
        prov:wasInfluencedBy  <https://wiki.openstreetmap.org/wiki/Key:barrier> .

osm:ConstructionValue
        a                     rdfs:Class , owl:Class ;
        rdfs:comment          "Used to describe a feature which is currently under construction."@en ;
        rdfs:label            "ConstructionValue"@en ;
        rdfs:isDefinedBy      osm: ;
        prov:wasInfluencedBy  <https://wiki.openstreetmap.org/wiki/Key:construction> .

osm:CrossingValue
        a                     rdfs:Class , owl:Class ;
        rdfs:comment          "This tag is used for more accurately describing specific types of pedestrian crossings."@en ;
        rdfs:label            "CrossingValue"@en ;
        rdfs:isDefinedBy      osm: ;
        prov:wasInfluencedBy  <https://wiki.openstreetmap.org/wiki/Key:crossing> .

osm:CyclewayValue
        a                     rdfs:Class , owl:Class ;
        rdfs:comment          "Maps cycling infrastructure that is an inherent part of the road."@en ;
        rdfs:label            "CyclewayValue"@en ;
        rdfs:isDefinedBy      osm: ;
        prov:wasInfluencedBy  <https://wiki.openstreetmap.org/wiki/Key:cycleway> .

osm:FootwayValue
        a                     rdfs:Class , owl:Class ;
        rdfs:comment          "Refines the osm:Footway for sidewalks."@en ;
        rdfs:label            "FootwayValue"@en ;
        rdfs:isDefinedBy      osm: ;
        prov:wasInfluencedBy  <https://wiki.openstreetmap.org/wiki/Key:footway> .

osm:HighwayValue
        a                     rdfs:Class , owl:Class ;
        rdfs:comment          "Indicates the role and importance of the way within the road network."@en ;
        rdfs:label            "HighwayValue"@en ;
        rdfs:isDefinedBy      osm: ;
        prov:wasInfluencedBy  <https://wiki.openstreetmap.org/wiki/Key:highway> .

osm:MotorroadValue
        a                     rdfs:Class , owl:Class ;
        rdfs:comment          "Describe highways that have motorway-like access restrictions but that are not a motorway."@en ;
        rdfs:label            "MotorroadValue"@en ;
        rdfs:isDefinedBy      osm: ;
        prov:wasInfluencedBy  <https://wiki.openstreetmap.org/wiki/Key:motorroad> .

osm:MtbScaleValue
        a                     rdfs:Class , owl:Class ;
        rdfs:comment          "Provides a classification scheme for mapping the difficulty of trails suitable for mountain-biking."@en ;
        rdfs:label            "MtbScaleValue"@en ;
        rdfs:isDefinedBy      osm: ;
        prov:wasInfluencedBy  <https://wiki.openstreetmap.org/wiki/Key:mtb:scale> .

osm:OnewayValue
        a                     rdfs:Class , owl:Class ;
        rdfs:comment          "Indicate the access restriction on highways and other linear features."@en ;
        rdfs:label            "OnewayValue"@en ;
        rdfs:isDefinedBy      osm: ;
        prov:wasInfluencedBy  <https://wiki.openstreetmap.org/wiki/Key:oneway> .

osm:SegregatedValue
        a                     rdfs:Class , owl:Class ;
        rdfs:comment          "Used for combined cycle- and footways."@en ;
        rdfs:label            "SegregatedValue"@en ;
        rdfs:isDefinedBy      osm: ;
        prov:wasInfluencedBy  <https://wiki.openstreetmap.org/wiki/Key:segregated> .

osm:SmoothnessValue
        a                     rdfs:Class , owl:Class ;
        rdfs:comment          "Provides a classification scheme regarding the physical usability of a way."@en ;
        rdfs:label            "SmoothnessValue"@en ;
        rdfs:isDefinedBy      osm: ;
        prov:wasInfluencedBy  <https://wiki.openstreetmap.org/wiki/Key:smoothness> .

osm:SurfaceValue
        a                     rdfs:Class , owl:Class ;
        rdfs:comment          "Provides information about the physical surface of elements, particularly regarding material composition and/or structure."@en ;
        rdfs:label            "SurfaceValue"@en ;
        rdfs:isDefinedBy      osm: ;
        prov:wasInfluencedBy  <https://wiki.openstreetmap.org/wiki/Key:surface> .

osm:TracktypeValue
        a                     rdfs:Class , owl:Class ;
        rdfs:comment          "Measures how well-maintained a track is, particularly regarding surface firmness."@en ;
        rdfs:label            "TracktypeValue"@en ;
        rdfs:isDefinedBy      osm: ;
        prov:wasInfluencedBy  <https://wiki.openstreetmap.org/wiki/Key:tracktype> .

# Individuals

## Access

osm:Agricultural  
        a                     osm:AccessValue ;
        rdfs:comment          "Only for agricultural traffic."@en ;
        rdfs:label            "access=agricultural"@en ;
        rdfs:isDefinedBy      osm: ;
        prov:wasInfluencedBy  <https://wiki.openstreetmap.org/wiki/Key:access> .

osm:Customers  
        a                     osm:AccessValue ;
        rdfs:comment          "Only for customers of the element."@en ;
        rdfs:label            "access=customers"@en ;
        rdfs:isDefinedBy      osm: ;
        prov:wasInfluencedBy  <https://wiki.openstreetmap.org/wiki/Key:access> .

osm:Delivery  
        a                     osm:AccessValue ;
        rdfs:comment          "Only when delivering to the element."@en ;
        rdfs:label            "access=customers"@en ;
        rdfs:isDefinedBy      osm: ;
        prov:wasInfluencedBy  <https://wiki.openstreetmap.org/wiki/Key:access> .

osm:Designated  
        a                     osm:AccessValue ;
        rdfs:comment          "A preferred or designated route."@en ;
        rdfs:label            "access=designated"@en ;
        rdfs:isDefinedBy      osm: ;
        prov:wasInfluencedBy  <https://wiki.openstreetmap.org/wiki/Key:access> .

osm:Destination  
        a                     osm:AccessValue ;
        rdfs:comment          "Only when travelling to this element/area; i.e., local traffic only."@en ;
        rdfs:label            "access=destination"@en ;
        rdfs:isDefinedBy      osm: ;
        prov:wasInfluencedBy  <https://wiki.openstreetmap.org/wiki/Key:access> .

osm:Discouraged  
        a                     osm:AccessValue ;
        rdfs:comment          "A legal right of way exists but usage is officially discouraged."@en ;
        rdfs:label            "access=discouraged"@en ;
        rdfs:isDefinedBy      osm: ;
        prov:wasInfluencedBy  <https://wiki.openstreetmap.org/wiki/Key:access> .

osm:Dismount  
        a                     osm:AccessValue ;
        rdfs:comment          "Permitted for some vehicle (or animal) only if you dismount."@en ;
        rdfs:label            "access=dismount"@en ;
        rdfs:isDefinedBy      osm: ;
        prov:wasInfluencedBy  <https://wiki.openstreetmap.org/wiki/Key:access> .

osm:Emergency  
        a                     osm:AccessValue ;
        rdfs:comment          "Only for emergency vehicles."@en ;
        rdfs:label            "access=emergency"@en ;
        rdfs:isDefinedBy      osm: .

osm:Forestry  
        a                     osm:AccessValue ;
        rdfs:comment          "Only for forestry traffic."@en ;
        rdfs:label            "access=forestry"@en ;
        rdfs:isDefinedBy      osm: ;
        prov:wasInfluencedBy  <https://wiki.openstreetmap.org/wiki/Key:access> .

osm:FreeAccess  
        a                     osm:AccessValue ;
        rdfs:comment          "The public has an official, legally-enshrined right of access; i.e., it's a right of way."@en ;
        rdfs:label            "access=yes"@en ;
        rdfs:isDefinedBy      osm: ;
        prov:wasInfluencedBy  <https://wiki.openstreetmap.org/wiki/Key:access> .

osm:NoAccess  
        a                     osm:AccessValue ;
        rdfs:comment          "No access for the general public."@en ;
        rdfs:label            "access=no"@en ;
        rdfs:isDefinedBy      osm: ;
        prov:wasInfluencedBy  <https://wiki.openstreetmap.org/wiki/Key:access> .

osm:OfficialAccess  
        a                     osm:AccessValue ;
        rdfs:comment          "A way legally dedicated to specific modes of travel by a law or by the rules of traffic."@en ;
        rdfs:label            "access=official"@en ;
        rdfs:isDefinedBy      osm: ;
        prov:wasInfluencedBy  <https://wiki.openstreetmap.org/wiki/Tag:access%3Dofficial> .

osm:Permissive  
        a                     osm:AccessValue ;
        rdfs:comment          "Open to general traffic until such time as the owner revokes the permission."@en ;
        rdfs:label            "access=permissive"@en ;
        rdfs:isDefinedBy      osm: ;
        prov:wasInfluencedBy  <https://wiki.openstreetmap.org/wiki/Key:access> .

osm:Private  
        a                     osm:AccessValue ;
        rdfs:comment          "Only with individual permission."@en ;
        rdfs:label            "access=private"@en ;
        rdfs:isDefinedBy      osm: ;
        prov:wasInfluencedBy  <https://wiki.openstreetmap.org/wiki/Key:access> .

osm:UseSidepath  
        a                     osm:AccessValue ;
        rdfs:comment          "Can only be used in countries with compulsory cycleways and gives access information on parallel roads."@en ;
        rdfs:label            "access=use_sidepath"@en ;
        rdfs:isDefinedBy      osm: ;
        prov:wasInfluencedBy  <https://wiki.openstreetmap.org/wiki/Key:access> .

## Barrier

osm:Block  
        a                     osm:BarrierValue ;
        rdfs:comment          "A large, solid, immobile block that can be moved only with heavy machinery or great effort."@en ;
        rdfs:label            "barrier=block"@en ;
        rdfs:isDefinedBy      osm: ;
        prov:wasInfluencedBy  <https://wiki.openstreetmap.org/wiki/Key:barrier> .

osm:Bollard  
        a                     osm:BarrierValue ;
        rdfs:comment          "Solid (usually concrete or metal) pillar or pillars in the middle of the road to prevent passage by some traffic."@en ;
        rdfs:label            "barrier=bollard"@en ;
        rdfs:isDefinedBy      osm: ;
        prov:wasInfluencedBy  <https://wiki.openstreetmap.org/wiki/Key:bollard> .

osm:BorderControl  
        a                     osm:BarrierValue ;
        rdfs:comment          "This is a control point at an international border between two countries. Passports or other forms of ID will be checked."@en ;
        rdfs:label            "barrier=border_control"@en ;
        rdfs:isDefinedBy      osm: ;
        prov:wasInfluencedBy  <https://wiki.openstreetmap.org/wiki/Key:border_control> .

osm:BumpGate  
        a                     osm:BarrierValue ;
        rdfs:comment          "A bump gate is a drive-through gate used in rural areas to provide a barrier to livestock that does not require the driver to exit the vehicle."@en ;
        rdfs:label            "barrier=bump_gate"@en ;
        rdfs:isDefinedBy      osm: ;
        prov:wasInfluencedBy  <https://en.wikipedia.org/wiki/Bump_gate> .

osm:BusTrap  
        a                     osm:BarrierValue ;
        rdfs:comment          "A bus trap is a metal grate placed over a ditch or pit in the road with tines (sides) spaced far enough apart that small-diameter-wheeled (narrower axle) vehicles fall in between the tines but close enough that larger-diameter-wheeled vehicles, such as buses, may pass."@en ;
        rdfs:label            "barrier=bus_trap"@en ;
        rdfs:isDefinedBy      osm: ;
        prov:wasInfluencedBy  <https://en.wikipedia.org/wiki/Bus_trap> .

osm:CattleGrid  
        a                     osm:BarrierValue ;
        rdfs:comment          "Bars in the road surface that allow wheeled vehicles but not animals to cross."@en ;
        rdfs:label            "barrier=cattle_grid"@en ;
        rdfs:isDefinedBy      osm: ;
        prov:wasInfluencedBy  <https://wiki.openstreetmap.org/wiki/Key:barrier> .

osm:Chain  
        a                     osm:BarrierValue ;
        rdfs:comment          "A chain used to prevent motorised vehicles."@en ;
        rdfs:label            "barrier=chain"@en ;
        rdfs:isDefinedBy      osm: ;
        prov:wasInfluencedBy  <https://wiki.openstreetmap.org/wiki/Key:barrier> .

osm:CycleBarrier  
        a                     osm:BarrierValue ;
        rdfs:comment          "Barriers to bicycle traffic, most typically a pair of staggered steel bars perpendicular to the way itself whose gaps allow pedestrians to pass."@en ;
        rdfs:label            "barrier=cycle_barrier"@en ;
        rdfs:isDefinedBy      osm: ;
        prov:wasInfluencedBy  <https://wiki.openstreetmap.org/wiki/Key:barrier> .

osm:Debris  
        a                     osm:BarrierValue ;
        rdfs:comment          "A road is blocked by debris with or without ground. This might be for short or long time. Often used as first step in blocking an abandoned road."@en ;
        rdfs:label            "barrier=debris"@en ;
        rdfs:isDefinedBy      osm: ;
        prov:wasInfluencedBy  <https://wiki.openstreetmap.org/wiki/Key:barrier> .

osm:Entrance  
        a                     osm:BarrierValue ;
        rdfs:comment          "A gap in a linear barrier with nothing that limits passing through."@en ;
        rdfs:label            "barrier=entrance"@en ;
        rdfs:isDefinedBy      osm: ;
        prov:wasInfluencedBy  <https://wiki.openstreetmap.org/wiki/Key:barrier> .

osm:Gate  
        a                     osm:BarrierValue ;
        rdfs:comment          "An entrance that can be opened or closed to get through the barrier."@en ;
        rdfs:label            "barrier=gate"@en ;
        rdfs:isDefinedBy      osm: ;
        prov:wasInfluencedBy  <https://wiki.openstreetmap.org/wiki/Key:barrier> .

osm:LiftGate  
        a                     osm:BarrierValue ;
        rdfs:comment          "A lift gate (boom barrier) is a bar, or pole pivoted in such a way as to allow the boom to block vehicular access through a controlled point."@en ;
        rdfs:label            "barrier=lift_gate"@en ;
        rdfs:isDefinedBy      osm: ;
        prov:wasInfluencedBy  <https://wiki.openstreetmap.org/wiki/Key:barrier> .

osm:SallyPort  
        a                     osm:BarrierValue ;
        rdfs:comment          "A sally port is used to pass through thick or city walls, and is a type of covered gate with two doors."@en ;
        rdfs:label            "barrier=sally_port"@en ;
        rdfs:isDefinedBy      osm: ;
        prov:wasInfluencedBy  <https://wiki.openstreetmap.org/wiki/Key:barrier> .

osm:SwingGate  
        a                     osm:BarrierValue ;
        rdfs:comment          "Similar to a lift gate but rotates sidewards to open."@en ;
        rdfs:label            "barrier=swing_gate"@en ;
        rdfs:isDefinedBy      osm: ;
        prov:wasInfluencedBy  <https://wiki.openstreetmap.org/wiki/Key:barrier> .

osm:TollBooth  
        a                     osm:BarrierValue ;
        rdfs:comment          "A road usage toll or fee is collected here."@en ;
        rdfs:label            "barrier=toll_booth"@en ;
        rdfs:isDefinedBy      osm: ;
        prov:wasInfluencedBy  <https://wiki.openstreetmap.org/wiki/Key:barrier> .

osm:Turnstile  
        a                     osm:BarrierValue ;
        rdfs:comment          "A turnstile (also called baffle gate) is used to allow one person at a time to pass."@en ;
        rdfs:label            "barrier=turnstile"@en ;
        rdfs:isDefinedBy      osm: ;
        prov:wasInfluencedBy  <https://wiki.openstreetmap.org/wiki/Key:barrier> .

## Construction

osm:UnderConstruction  
        a                     osm:ConstructionValue ;
        rdfs:comment          "Indicates that this element is under construction."@en ;
        rdfs:label            "construction=yes"@en ;
        rdfs:isDefinedBy      osm: ;
        prov:wasInfluencedBy  <https://wiki.openstreetmap.org/wiki/Tag%3Aconstruction%3Dyes> .

## Crossing

osm:Uncontrolled  
        a                     osm:CrossingValue ;
        rdfs:comment          "A generic crossing with no traffic-signals of any type, just road markings."@en ;
        rdfs:label            "crossing=uncontrolled"@en ;
        rdfs:isDefinedBy      osm: ;
        prov:wasInfluencedBy  <https://wiki.openstreetmap.org/wiki/Key:crossing> .

osm:Unmarked  
        a                     osm:CrossingValue ;
        rdfs:comment          "A crossing without road markings or traffic lights"@en ;
        rdfs:label            "crossing=unmarked"@en ;
        rdfs:isDefinedBy      osm: ;
        prov:wasInfluencedBy  <https://wiki.openstreetmap.org/wiki/Key:crossing> .

## Cycleway

osm:Lane  
        a                     osm:CyclewayValue ;
        rdfs:comment          "Two-way streets where there are cycle lanes on both sides of the road."@en ;
        rdfs:label            "cycleway=lane"@en ;
        rdfs:isDefinedBy      osm: ;
        prov:wasInfluencedBy  <https://wiki.openstreetmap.org/wiki/Tag%3Acycleway%3Dlane> .

osm:Opposite  
        a                     osm:CyclewayValue ;
        rdfs:comment          "Cyclists are permitted to travel in both directions on a road which is one-way for normal traffic."@en ;
        rdfs:label            "cycleway=opposite"@en ;
        rdfs:isDefinedBy      osm: ;
        prov:wasInfluencedBy  <https://wiki.openstreetmap.org/wiki/Tag%3Acycleway%3Dopposite> .

osm:OppositeLane
        a                     osm:CyclewayValue ;
        rdfs:comment          "A one-way street that has a cycling lane going in the opposite direction to normal traffic flow."@en ;
        rdfs:label            "cycleway=opposite_lane"@en ;
        rdfs:isDefinedBy      osm: ;
        prov:wasInfluencedBy  <https://wiki.openstreetmap.org/wiki/Tag%3Acycleway%3Dopposite_lane> .

osm:OppositeTrack
        a                     osm:CyclewayValue ;
        rdfs:comment          "A cycle track travelling in the opposite direction to other traffic."@en ;
        rdfs:label            "cycleway=opposite_track"@en ;
        rdfs:isDefinedBy      osm: ;
        prov:wasInfluencedBy  <https://wiki.openstreetmap.org/wiki/Tag%3Acycleway%3Dopposite_track> .

osm:ShareBusway
        a                     osm:CyclewayValue ;
        rdfs:comment          "A cycle lane taking the form of a bus lane that is also designated for use by cyclists."@en ;
        rdfs:label            "cycleway=share_busway"@en ;
        rdfs:isDefinedBy      osm: ;
        prov:wasInfluencedBy  <https://wiki.openstreetmap.org/wiki/Tag%3Acycleway%3Dshare_busway> .

osm:Shared
        a                     osm:CyclewayValue ;
        rdfs:comment          "In general, this indicates that cyclists share space with other traffic on this highway."@en ;
        rdfs:label            "cycleway=shared"@en ;
        rdfs:isDefinedBy      osm: ;
        prov:wasInfluencedBy  <https://wiki.openstreetmap.org/wiki/Key:cycleway> .

osm:SharedLane
        a                     osm:CyclewayValue ;
        rdfs:comment          "Roads which contain a shared lane marking, or sharrow, to indicate that the travel lane is shared by bicycles and other vehicles."@en ;
        rdfs:label            "cycleway=shared_lane"@en ;
        rdfs:isDefinedBy      osm: ;
        prov:wasInfluencedBy  <https://wiki.openstreetmap.org/wiki/Proposed_features/shared_lane> .

## Footway

osm:Sidewalk
        a                     osm:FootwayValue ;
        rdfs:comment          "A sidewalk that's distinct from the carriageway."@en ;
        rdfs:label            "footway=sidewalk"@en ;
        rdfs:isDefinedBy      osm: ;
        prov:wasInfluencedBy  <https://wiki.openstreetmap.org/wiki/Tag%3Afootway%3Dsidewalk> .

## Highway

osm:Bridleway  
        a                     osm:HighwayValue ;
        rdfs:comment          "A way intended for use by horse riders."@en ;
        rdfs:label            "highway=bridleway"@en ;
        rdfs:isDefinedBy      osm: ;
        prov:wasInfluencedBy  <https://wiki.openstreetmap.org/wiki/Tag%3Ahighway%3Dbridleway> .

osm:CycleHighway  
        a                     osm:HighwayValue ;
        owl:sameAs            <http://www.wikidata.org/entity/Q1628979> ;
        rdfs:comment          "For designated cycleways."@en ;
        rdfs:label            "highway=cycleway"@en ;
        rdfs:isDefinedBy      osm: ;
        prov:wasInfluencedBy  <https://wiki.openstreetmap.org/wiki/Key:highway> .

osm:FootHighway  
        a                     osm:HighwayValue ;
        owl:sameAs            <http://www.wikidata.org/entity/Q3352369> ;
        rdfs:comment          "Designated footpaths; i.e., mainly/exclusively for pedestrians."@en ;
        rdfs:label            "highway=footway"@en ;
        rdfs:isDefinedBy      osm: ;
        prov:wasInfluencedBy  <https://wiki.openstreetmap.org/wiki/Key:highway> .

osm:HighwayCrossing  
        a                     osm:HighwayValue ;
        owl:sameAs            <http://www.wikidata.org/entity/Q8010> ;
        rdfs:comment          "Pedestrians can cross a street here."@en ;
        rdfs:label            "highway=crossing"@en ;
        rdfs:isDefinedBy      osm: ;
        prov:wasInfluencedBy  <https://wiki.openstreetmap.org/wiki/Tag%3Ahighway%3Dcrossing> .

osm:GiveWay  
        a                     osm:HighwayValue ;
        rdfs:comment          "Points where a traffic sign instructs traffic to cede priority."@en ;
        rdfs:label            "highway=give_way"@en ;
        rdfs:isDefinedBy      osm: ;
        prov:wasInfluencedBy  <https://wiki.openstreetmap.org/wiki/Tag%3Ahighway%3Dgive_way> .

osm:LivingStreet  
        a                     osm:HighwayValue ;
        owl:sameAs            <http://www.wikidata.org/entity/Q1628979> ;
        rdfs:comment          "For living streets, which are residential streets where pedestrians have legal priority over cars."@en ;
        rdfs:label            "highway=living_street"@en ;
        rdfs:isDefinedBy      osm: ;
        prov:wasInfluencedBy  <https://wiki.openstreetmap.org/wiki/Key:highway> .

osm:Motorway  
        a                     osm:HighwayValue ;
        owl:sameAs            <http://www.wikidata.org/entity/Q46622> ;
        rdfs:comment          "A restricted access major divided highway, normally with 2 or more running lanes plus emergency hard shoulder."@en ;
        rdfs:label            "highway=motorway"@en ;
        rdfs:isDefinedBy      osm: ;
        prov:wasInfluencedBy  <https://wiki.openstreetmap.org/wiki/Key:highway> .

osm:MotorwayLink  
        a                     osm:HighwayValue ;
        rdfs:comment          "The link roads leading to/from a motorway."@en ;
        rdfs:label            "highway=motorway_link"@en ;
        rdfs:isDefinedBy      osm: ;
        prov:wasInfluencedBy  <https://wiki.openstreetmap.org/wiki/Key:highway> .

osm:Path  
        a                     osm:HighwayValue ;
        rdfs:comment          "A non-specific path."@en ;
        rdfs:label            "highway=path"@en ;
        rdfs:isDefinedBy      osm: ;
        prov:wasInfluencedBy  <https://wiki.openstreetmap.org/wiki/Key:highway> .    

osm:Primary  
        a                     osm:HighwayValue ;
        rdfs:comment          "The next most important roads in a country's system, after trunks."@en ;
        rdfs:label            "highway=primary"@en ;
        rdfs:isDefinedBy      osm: ;
        prov:wasInfluencedBy  <https://wiki.openstreetmap.org/wiki/Key:highway> .

osm:PrimaryLink  
        a                     osm:HighwayValue ;
        rdfs:comment          "The link roads leading to/from a primary road."@en ;
        rdfs:label            "highway=primary_link"@en ;
        rdfs:isDefinedBy      osm: ;
        prov:wasInfluencedBy  <https://wiki.openstreetmap.org/wiki/Key:highway> .

osm:Proposed  
        a                     osm:HighwayValue ;
        rdfs:comment          "For roads that are about to be built, but where any construction work hasn't yet been started."@en ;
        rdfs:label            "highway=proposed"@en ;
        rdfs:isDefinedBy      osm: ;
        prov:wasInfluencedBy  <https://wiki.openstreetmap.org/wiki/Tag%3Ahighway%3Dproposed> .

osm:Residential  
        a                     osm:HighwayValue ;
        rdfs:comment          "Roads which serve as an access to housing, without function of connecting settlements. Often lined with housing."@en ;
        rdfs:label            "highway=residential"@en ;
        rdfs:isDefinedBy      osm: ;
        prov:wasInfluencedBy  <https://wiki.openstreetmap.org/wiki/Key:highway> .

osm:Road  
        a                     osm:HighwayValue ;
        rdfs:comment          "This tag is used for a road with an unknown classification."@en ;
        rdfs:label            "highway=road"@en ;
        rdfs:isDefinedBy      osm: ;
        prov:wasInfluencedBy  <https://wiki.openstreetmap.org/wiki/Tag%3Ahighway%3Droad> .

osm:Secondary  
        a                     osm:HighwayValue ;
        rdfs:comment          "The next most important roads in a country's system, after primary roads."@en ;
        rdfs:label            "highway=secondary"@en ;
        rdfs:isDefinedBy      osm: ;
        prov:wasInfluencedBy  <https://wiki.openstreetmap.org/wiki/Key:highway> .

osm:SecondaryLink  
        a                     osm:HighwayValue ;
        rdfs:comment          "The link roads leading to/from a secondary road."@en ;
        rdfs:label            "highway=secondary_link"@en ;
        rdfs:isDefinedBy      osm: ;
        prov:wasInfluencedBy  <https://wiki.openstreetmap.org/wiki/Key:highway> .

osm:Service  
        a                     osm:HighwayValue ;
        rdfs:comment          "For access roads to, or within an industrial estate, camp site, business park, car park etc."@en ;
        rdfs:label            "highway=service"@en ;
        rdfs:isDefinedBy      osm: ;
        prov:wasInfluencedBy  <https://wiki.openstreetmap.org/wiki/Key:highway> .

osm:Steps  
        a                     osm:HighwayValue ;
        owl:sameAs            <http://www.wikidata.org/entity/Q12511> ;
        rdfs:comment          "Flights of steps on footways and paths."@en ;
        rdfs:label            "highway=steps"@en ;
        rdfs:isDefinedBy      osm: ;
        prov:wasInfluencedBy  <https://wiki.openstreetmap.org/wiki/Tag%3Ahighway%3Dsteps> .

osm:Stop  
        a                     osm:HighwayValue ;
        rdfs:comment          "Points at which vehicles are required to stop."@en ;
        rdfs:label            "highway=stop"@en ;
        rdfs:isDefinedBy      osm: ;
        prov:wasInfluencedBy  <https://wiki.openstreetmap.org/wiki/Tag%3Ahighway%3Dstop> .

osm:Tertiary  
        a                     osm:HighwayValue ;
        rdfs:comment          "The next most important roads in a country's system, after secondary roads."@en ;
        rdfs:label            "highway=tertiary"@en ;
        rdfs:isDefinedBy      osm: ;
        prov:wasInfluencedBy  <https://wiki.openstreetmap.org/wiki/Key:highway> .

osm:TertiaryLink  
        a                     osm:HighwayValue ;
        rdfs:comment          "The link roads leading to/from a tertiary road."@en ;
        rdfs:label            "highway=tertiary_link"@en ;
        rdfs:isDefinedBy      osm: ;
        prov:wasInfluencedBy  <https://wiki.openstreetmap.org/wiki/Key:highway> .

osm:Track  
        a                     osm:HighwayValue ;
        rdfs:comment          "Roads for mostly agricultural or forestry uses. If used in the context of a cycleway this means a cycle track running parallel to a road."@en ;
        rdfs:label            "highway=track"@en ;
        rdfs:isDefinedBy      osm: ;
        prov:wasInfluencedBy  <https://wiki.openstreetmap.org/wiki/Key:highway> .

osm:TrafficSignals  
        a                     osm:HighwayValue ;
        rdfs:comment          "Signalling devices positioned at road intersections, pedestrian crossings and other locations to control competing flows of traffic. "@en ;
        rdfs:label            "highway=traffic_signals"@en ;
        rdfs:isDefinedBy      osm: ;
        prov:wasInfluencedBy  <https://wiki.openstreetmap.org/wiki/Tag%3Ahighway%3Dtraffic_signals> .

osm:Trunk  
        a                     osm:HighwayValue ;
        owl:sameAs            <http://www.wikidata.org/entity/Q1302778> ;
        rdfs:comment          "The most important roads in a country's system that aren't motorways."@en ;
        rdfs:label            "highway=trunk"@en ;
        rdfs:isDefinedBy      osm: ;
        prov:wasInfluencedBy  <https://wiki.openstreetmap.org/wiki/Key:highway> .

osm:TrunkLink  
        a                     osm:HighwayValue ;
        rdfs:comment          "The link roads leading to/from a trunk road."@en ;
        rdfs:label            "highway=trunk_link"@en ;
        rdfs:isDefinedBy      osm: ;
        prov:wasInfluencedBy  <https://wiki.openstreetmap.org/wiki/Key:highway> .

osm:Unclassified  
        a                     osm:HighwayValue ;
        rdfs:comment          "The least important through roads in a country's system."@en ;
        rdfs:label            "highway=unclassified"@en ;
        rdfs:isDefinedBy      osm: ;
        prov:wasInfluencedBy  <https://wiki.openstreetmap.org/wiki/Key:highway> .


## Oneway

osm:Bidirectional  
        a                     osm:OnewayValue ;
        rdfs:comment          "This is not a oneway street."@en ;
        rdfs:label            "oneway=no"@en ;
        rdfs:isDefinedBy      osm: ;
        prov:wasInfluencedBy  <https://wiki.openstreetmap.org/wiki/Key:oneway> .

osm:InOrder  
        a                     osm:OnewayValue ;
        rdfs:comment          "This is a oneway street, with the direction being the same order of the way nodes."@en ;
        rdfs:label            "oneway=yes"@en ;
        rdfs:isDefinedBy      osm: ;
        prov:wasInfluencedBy  <https://wiki.openstreetmap.org/wiki/Key:oneway> .

osm:InReverseOrder  
        a                     osm:OnewayValue ;
        rdfs:comment          "This is a oneway street, with the direction being the reverse of the order of the way nodes."@en ;
        rdfs:label            "oneway=-1"@en ;
        rdfs:isDefinedBy      osm: ;
        prov:wasInfluencedBy  <https://wiki.openstreetmap.org/wiki/Key:oneway> .


## Smoothness

osm:ExcellentSmoothness  
        a                     osm:SmoothnessValue ;
        rdfs:comment          "Usable by roller blades, skate boards and everything that can use roads with 'good' smoothness."@en ;
        rdfs:label            "smoothness=excellent"@en ;
        rdfs:isDefinedBy      osm: ;
        prov:wasInfluencedBy  <https://wiki.openstreetmap.org/wiki/Key:smoothness> .

osm:GoodSmoothness  
        a                     osm:SmoothnessValue ;
        rdfs:comment          "Usable by racing bikes and everything that can use roads with 'intermediate' smoothness."@en ;
        rdfs:label            "smoothness=good"@en ;
        rdfs:isDefinedBy      osm: ;
        prov:wasInfluencedBy  <https://wiki.openstreetmap.org/wiki/Key:smoothness> .

osm:IntermediateSmoothness  
        a                     osm:SmoothnessValue ;
        rdfs:comment          "Usable by city bikes, sport cars, wheel chairs and everything that can use roads with 'bad' smoothness."@en ;
        rdfs:label            "smoothness=intermediate"@en ;
        rdfs:isDefinedBy      osm: ;
        prov:wasInfluencedBy  <https://wiki.openstreetmap.org/wiki/Key:smoothness> .

osm:BadSmoothness  
        a                     osm:SmoothnessValue ;
        rdfs:comment          "Usable by trekking bikes, normal cars and everything that can use roads with 'very bad' smoothness."@en ;
        rdfs:label            "smoothness=bad"@en ;
        rdfs:isDefinedBy      osm: ;
        prov:wasInfluencedBy  <https://wiki.openstreetmap.org/wiki/Key:smoothness> .

osm:VeryBadSmoothness  
        a                     osm:SmoothnessValue ;
        rdfs:comment          "Usable by cars with high clearance, light-duty off-road vehicles and everything that can use roads with 'horrible' smoothness."@en ;
        rdfs:label            "smoothness=very_bad"@en ;
        rdfs:isDefinedBy      osm: ;
        prov:wasInfluencedBy  <https://wiki.openstreetmap.org/wiki/Key:smoothness> .

osm:HorribleSmoothness  
        a                     osm:SmoothnessValue ;
        rdfs:comment          "Usable by heavy-duty off-road vehicles and everything that can use roads with 'very horrible' smoothness."@en ;
        rdfs:label            "smoothness=horrible"@en ;
        rdfs:isDefinedBy      osm: ;
        prov:wasInfluencedBy  <https://wiki.openstreetmap.org/wiki/Key:smoothness> .

osm:VeryHorribleSmoothness  
        a                     osm:SmoothnessValue ;
        rdfs:comment          "Usable by tractors, ATVs and tanks."@en ;
        rdfs:label            "smoothness=very_horrible"@en ;
        rdfs:isDefinedBy      osm: ;
        prov:wasInfluencedBy  <https://wiki.openstreetmap.org/wiki/Key:smoothness> .

osm:ImpassableSmoothness  
        a                     osm:SmoothnessValue ;
        rdfs:comment          "Not usable by wheeled vehicles."@en ;
        rdfs:label            "smoothness=impassable"@en ;
        rdfs:isDefinedBy      osm: ;
        prov:wasInfluencedBy  <https://wiki.openstreetmap.org/wiki/Key:smoothness> .


## Surface

osm:Asphalt  
        a                     osm:SurfaceValue ;
        owl:sameAs            <http://www.wikidata.org/entity/Q189259> ;
        rdfs:comment          "This road has an asphalt surface."@en ;
        rdfs:label            "surface=asphalt"@en ;
        rdfs:isDefinedBy      osm: ;
        prov:wasInfluencedBy  <https://wiki.openstreetmap.org/wiki/Tag%3Asurface%3Dasphalt> .

osm:Cobblestone  
        a                     osm:SurfaceValue ;
        rdfs:comment          "This road has an cobblestone surface."@en ;
        rdfs:label            "surface=cobblestone"@en ;
        rdfs:isDefinedBy      osm: ;
        prov:wasInfluencedBy  <https://wiki.openstreetmap.org/wiki/Key:surface> .

osm:Compacted  
        a                     osm:SurfaceValue ;
        rdfs:comment          "A mixture of larger (e.g., gravel) and smaller (e.g., sand) parts, compacted so the surface is more stable than loose gravel."@en ;
        rdfs:label            "surface=compacted"@en ;
        rdfs:isDefinedBy      osm: ;
        prov:wasInfluencedBy  <https://wiki.openstreetmap.org/wiki/Tag%3Asurface%3Dcompacted> .

osm:Concrete  
        a                     osm:SurfaceValue ;
        rdfs:comment          "Cement based concrete."@en ;
        rdfs:label            "surface=concrete"@en ;
        rdfs:isDefinedBy      osm: ;
        prov:wasInfluencedBy  <https://wiki.openstreetmap.org/wiki/Key:surface> .

osm:Dirt  
        a                     osm:SurfaceValue ;
        rdfs:comment          "This road's surface is just dirt (earth)."@en ;
        rdfs:label            "surface=dirt"@en ;
        rdfs:isDefinedBy      osm: ;
        prov:wasInfluencedBy  <https://wiki.openstreetmap.org/wiki/Key:surface> .

osm:FineGravel  
        a                     osm:SurfaceValue ;
        rdfs:comment          "A multilayer pavement with a stone or gravel basis and a topmost surface of firm, granular gravel."@en ;
        rdfs:label            "surface=fine_gravel"@en ;
        rdfs:isDefinedBy      osm: ;
        prov:wasInfluencedBy  <https://wiki.openstreetmap.org/wiki/Key:surface> .

osm:Grass  
        a                     osm:SurfaceValue ;
        rdfs:comment          "Grass covered ground."@en ;
        rdfs:label            "surface=grass"@en ;
        rdfs:isDefinedBy      osm: ;
        prov:wasInfluencedBy  <https://wiki.openstreetmap.org/wiki/Key:surface> .

osm:Gravel  
        a                     osm:SurfaceValue ;
        rdfs:comment          "Broken/crushed rock with sharp edges."@en ;
        rdfs:label            "surface=gravel"@en ;
        rdfs:isDefinedBy      osm: ;
        prov:wasInfluencedBy  <https://wiki.openstreetmap.org/wiki/Key:surface> .

osm:Ground  
        a                     osm:SurfaceValue ;
        rdfs:comment          "No special surface, the ground itself has marks of human or animal usage."@en ;
        rdfs:label            "surface=ground"@en ;
        rdfs:isDefinedBy      osm: ;
        prov:wasInfluencedBy  <https://wiki.openstreetmap.org/wiki/Key:surface> .

osm:Mud  
        a                     osm:SurfaceValue ;
        rdfs:comment          "Like the ground surface, but usually wet."@en ;
        rdfs:label            "surface=mud"@en ;
        rdfs:isDefinedBy      osm: ;
        prov:wasInfluencedBy  <https://wiki.openstreetmap.org/wiki/Key:surface> .

osm:Paved  
        a                     osm:SurfaceValue ;
        rdfs:comment          "A non-specific paved surface."@en ;
        rdfs:label            "surface=paved"@en ;
        rdfs:isDefinedBy      osm: ;
        prov:wasInfluencedBy  <https://wiki.openstreetmap.org/wiki/Key:surface> .

osm:PavingStones
        a                     osm:SurfaceValue ;
        rdfs:comment          "A relatively smooth surface paved with stones."@en ;
        rdfs:label            "surface=paving_stones"@en ;
        rdfs:isDefinedBy      osm: ;
        prov:wasInfluencedBy  <https://wiki.openstreetmap.org/wiki/Key:surface> .

osm:Pebblestone
        a                     osm:SurfaceValue ;
        rdfs:comment          "Loosely arranged smooth stones."@en ;
        rdfs:label            "surface=pebblestone"@en ;
        rdfs:isDefinedBy      osm: ;
        prov:wasInfluencedBy  <https://wiki.openstreetmap.org/wiki/Key:surface> .

osm:Sand
        a                     osm:SurfaceValue ;
        rdfs:comment          "Small to very small fractions of rock."@en ;
        rdfs:label            "surface=sand"@en ;
        rdfs:isDefinedBy      osm: ;
        prov:wasInfluencedBy  <https://wiki.openstreetmap.org/wiki/Key:surface> .

osm:Sett
        a                     osm:SurfaceValue ;
        rdfs:comment          "Sett paving, formed from natural stones cut to a regular shape. The stones do not cover the surface completely, unlike paving_stones."@en ;
        rdfs:label            "surface=sett"@en ;
        rdfs:isDefinedBy      osm: ;
        prov:wasInfluencedBy  <https://wiki.openstreetmap.org/wiki/Key:surface> .

osm:UnhewnCobblestone
        a                     osm:SurfaceValue ;
        rdfs:comment          "Cobblestone paving, formed from natural, uncut, overall rounded stones. Firmly attached to a ground, unlike pebblestone."@en ;
        rdfs:label            "surface=unhewn_cobblestone"@en ;
        rdfs:isDefinedBy      osm: ;
        prov:wasInfluencedBy  <https://wiki.openstreetmap.org/wiki/Key:surface> .

osm:Unpaved
        a                     osm:SurfaceValue ;
        rdfs:comment          "A loose covering ranging from compacted stone chippings to earth."@en ;
        rdfs:label            "surface=unpaved"@en ;
        rdfs:isDefinedBy      osm: ;
        prov:wasInfluencedBy  <https://wiki.openstreetmap.org/wiki/Key:surface> .

osm:Wood
        a                     osm:SurfaceValue ;
        rdfs:comment          "Wood."@en ;
        rdfs:label            "surface=wood"@en ;
        rdfs:isDefinedBy      osm: ;
        prov:wasInfluencedBy  <https://wiki.openstreetmap.org/wiki/Key:surface> .
