@prefix : <https://w3id.org/openstreetmap/terms#> .
@prefix owl: <http://www.w3.org/2002/07/owl#> .
@prefix rdf: <http://www.w3.org/1999/02/22-rdf-syntax-ns#> .
@prefix xml: <http://www.w3.org/XML/1998/namespace> .
@prefix xsd: <http://www.w3.org/2001/XMLSchema#> .
@prefix rdfs: <http://www.w3.org/2000/01/rdf-schema#> .
@base <https://w3id.org/openstreetmap/terms#> .

<https://w3id.org/openstreetmap/terms#> rdf:type owl:Ontology ;
                                         <http://creativecommons.org/ns#license> <https://creativecommons.org/licenses/by/4.0/> ;
                                         <http://purl.org/dc/terms/creator> <https://biblio.ugent.be/person/802002413821> ,
                                                                            <https://pietercolpaert.be/#me> ;
                                         <http://purl.org/dc/terms/description> "This ontology describes the OpenStreetMap data model."@en ;
                                         <http://purl.org/dc/terms/issued> "2019-06-13"^^xsd:date ;
                                         <http://purl.org/dc/terms/modified> "2019-06-13"^^xsd:date ;
                                         <http://purl.org/vocab/vann/preferredNamespacePrefix> "osm" ;
                                         <http://purl.org/vocab/vann/preferredNamespaceUri> "https://w3id.org/openstreetmap/terms#" ;
                                         rdfs:label "OpenStreetMaps Vocabulary"@en .

#################################################################
#    Annotation properties
#################################################################

###  http://qudt.org/schema/qudt/hasUnit
<http://qudt.org/schema/qudt/hasUnit> rdf:type owl:AnnotationProperty .


###  http://www.w3.org/ns/prov#wasInfluencedBy
<http://www.w3.org/ns/prov#wasInfluencedBy> rdf:type owl:AnnotationProperty .


###  http://xmlns.com/foaf/0.1/mbox
<http://xmlns.com/foaf/0.1/mbox> rdf:type owl:AnnotationProperty .


###  http://xmlns.com/foaf/0.1/name
<http://xmlns.com/foaf/0.1/name> rdf:type owl:AnnotationProperty .


###  http://xmlns.com/foaf/0.1/primaryTopic
<http://xmlns.com/foaf/0.1/primaryTopic> rdf:type owl:AnnotationProperty .


#################################################################
#    Object Properties
#################################################################

###  https://w3id.org/openstreetmap/terms#access
:access rdf:type owl:ObjectProperty ;
        rdfs:domain :Element ;
        rdfs:range :AccessValue ;
        rdfs:comment "The legal access for highways and other transportation networks."@en ;
        rdfs:isDefinedBy <https://w3id.org/openstreetmap/terms#> ;
        rdfs:label "access=*"@en ;
        <http://www.w3.org/ns/prov#wasInfluencedBy> <https://wiki.openstreetmap.org/wiki/Key:access> .


###  https://w3id.org/openstreetmap/terms#barrier
:barrier rdf:type owl:ObjectProperty ;
         rdfs:domain [ rdf:type owl:Class ;
                       owl:unionOf ( :Node
                                     :Way
                                   )
                     ] ;
         rdfs:range :BarrierValue ;
         rdfs:comment "A physical structure which blocks or impedes movement."@en ;
         rdfs:isDefinedBy <https://w3id.org/openstreetmap/terms#> ;
         rdfs:label "barrier=*"@en ;
         <http://www.w3.org/ns/prov#wasInfluencedBy> <https://wiki.openstreetmap.org/wiki/Key:barrier> .


###  https://w3id.org/openstreetmap/terms#bicycle
:bicycle rdf:type owl:ObjectProperty ;
         rdfs:domain [ rdf:type owl:Class ;
                       owl:unionOf ( :Node
                                     :Way
                                   )
                     ] ;
         rdfs:range :AccessValue ;
         rdfs:comment "The legal restrictions for bicycles."@en ;
         rdfs:isDefinedBy <https://w3id.org/openstreetmap/terms#> ;
         rdfs:label "bicycle=*"@en ;
         <http://www.w3.org/ns/prov#wasInfluencedBy> <https://wiki.openstreetmap.org/wiki/Key:bicycle> .


###  https://w3id.org/openstreetmap/terms#construction
:construction rdf:type owl:ObjectProperty ;
              rdfs:domain [ rdf:type owl:Class ;
                            owl:unionOf ( :Node
                                          :Way
                                        )
                          ] ;
              rdfs:range :ConstructionValue ;
              rdfs:comment "A feature which is currently under construction."@en ;
              rdfs:isDefinedBy <https://w3id.org/openstreetmap/terms#> ;
              rdfs:label "construction=*"@en ;
              <http://www.w3.org/ns/prov#wasInfluencedBy> <https://wiki.openstreetmap.org/wiki/Key:construction> .


###  https://w3id.org/openstreetmap/terms#crossing
:crossing rdf:type owl:ObjectProperty ;
          rdfs:domain [ rdf:type owl:Class ;
                        owl:unionOf ( :Node
                                      :Way
                                    )
                      ] ;
          rdfs:range :CrossingValue ;
          rdfs:comment "A specific type of pedestrian crossing."@en ;
          rdfs:isDefinedBy <https://w3id.org/openstreetmap/terms#> ;
          rdfs:label "crossing=*"@en ;
          <http://www.w3.org/ns/prov#wasInfluencedBy> <https://wiki.openstreetmap.org/wiki/Key:crossing> .


###  https://w3id.org/openstreetmap/terms#cycleway
:cycleway rdf:type owl:ObjectProperty ;
          rdfs:domain :Way ;
          rdfs:range :CyclewayValue ;
          rdfs:comment "Cycling infrastructure that is an inherent part of the road."@en ;
          rdfs:isDefinedBy <https://w3id.org/openstreetmap/terms#> ;
          rdfs:label "cycleway=*"@en ;
          <http://www.w3.org/ns/prov#wasInfluencedBy> <https://wiki.openstreetmap.org/wiki/Key:cycleway> .


###  https://w3id.org/openstreetmap/terms#footway
:footway rdf:type owl:ObjectProperty ;
         rdfs:domain :Way ;
         rdfs:range :FootwayValue ;
         rdfs:comment "A specific kind of footway."@en ;
         rdfs:isDefinedBy <https://w3id.org/openstreetmap/terms#> ;
         rdfs:label "footway=*"@en ;
         <http://www.w3.org/ns/prov#wasInfluencedBy> <https://wiki.openstreetmap.org/wiki/Key:footway> .


###  https://w3id.org/openstreetmap/terms#hasNodes
:hasNodes rdf:type owl:ObjectProperty ;
          rdfs:domain :Way ;
          rdfs:range rdf:list ;
          rdfs:comment """An ordered collection of nodes that describe the way. 
                              These may be fragmented over multiple predicates due to tiling for example.
                              Each fragment should have enough overlap to reconstruct the original way."""@en ;
          rdfs:isDefinedBy <https://w3id.org/openstreetmap/terms#> ;
          rdfs:label "hasNodes"@en .


###  https://w3id.org/openstreetmap/terms#highway
:highway rdf:type owl:ObjectProperty ;
         rdfs:domain [ rdf:type owl:Class ;
                       owl:unionOf ( :Node
                                     :Way
                                   )
                     ] ;
         rdfs:range :HighwayValue ;
         rdfs:comment "The kind of road, street or path."@en ;
         rdfs:isDefinedBy <https://w3id.org/openstreetmap/terms#> ;
         rdfs:label "highway=*"@en ;
         <http://www.w3.org/ns/prov#wasInfluencedBy> <https://wiki.openstreetmap.org/wiki/Key:highway> .


###  https://w3id.org/openstreetmap/terms#motor_vehicle
:motor_vehicle rdf:type owl:ObjectProperty ;
               rdfs:domain :Way ;
               rdfs:range :AccessValue ;
               rdfs:comment "The legal access restriction for all motor vehicles."@en ;
               rdfs:isDefinedBy <https://w3id.org/openstreetmap/terms#> ;
               rdfs:label "motor_vehicle=*"@en ;
               <http://www.w3.org/ns/prov#wasInfluencedBy> <https://wiki.openstreetmap.org/wiki/Key:motor_vehicle> .


###  https://w3id.org/openstreetmap/terms#motorcar
:motorcar rdf:type owl:ObjectProperty ;
          rdfs:domain :Way ;
          rdfs:range :AccessValue ;
          rdfs:comment "The legal access permission for cars."@en ;
          rdfs:isDefinedBy <https://w3id.org/openstreetmap/terms#> ;
          rdfs:label "motorcar=*"@en ;
          <http://www.w3.org/ns/prov#wasInfluencedBy> <https://wiki.openstreetmap.org/wiki/Key:motorcar> .


###  https://w3id.org/openstreetmap/terms#oneway
:oneway rdf:type owl:ObjectProperty ;
        rdfs:domain :Way ;
        rdfs:range :OnewayValue ;
        rdfs:comment "The direction restrictions on highways."@en ;
        rdfs:isDefinedBy <https://w3id.org/openstreetmap/terms#> ;
        rdfs:label "oneway=*"@en ;
        <http://www.w3.org/ns/prov#wasInfluencedBy> <https://wiki.openstreetmap.org/wiki/Key:oneway> .


###  https://w3id.org/openstreetmap/terms#oneway_bicycle
:oneway_bicycle rdf:type owl:ObjectProperty ;
                rdfs:domain :Way ;
                rdfs:range :OnewayValue ;
                rdfs:comment "The direction restrictions for cyclists specifically."@en ;
                rdfs:isDefinedBy <https://w3id.org/openstreetmap/terms#> ;
                rdfs:label "oneway:bicycle=*"@en ;
                <http://www.w3.org/ns/prov#wasInfluencedBy> <https://wiki.openstreetmap.org/wiki/Key:oneway:bicycle> .


###  https://w3id.org/openstreetmap/terms#smoothness
:smoothness rdf:type owl:ObjectProperty ;
            rdfs:domain :Way ;
            rdfs:range :SmoothnessValue ;
            rdfs:comment "A classification scheme regarding the physical usability of a way."@en ;
            rdfs:isDefinedBy <https://w3id.org/openstreetmap/terms#> ;
            rdfs:label "smoothness=*"@en ;
            <http://www.w3.org/ns/prov#wasInfluencedBy> <hhttps://wiki.openstreetmap.org/wiki/Key:smoothness> .


###  https://w3id.org/openstreetmap/terms#surface
:surface rdf:type owl:ObjectProperty ;
         rdfs:domain [ rdf:type owl:Class ;
                       owl:unionOf ( :Node
                                     :Way
                                   )
                     ] ;
         rdfs:range :SurfaceValue ;
         rdfs:comment "The physical surface of elements, particularly regarding material composition and/or structure."@en ;
         rdfs:isDefinedBy <https://w3id.org/openstreetmap/terms#> ;
         rdfs:label "surface=*"@en ;
         <http://www.w3.org/ns/prov#wasInfluencedBy> <https://wiki.openstreetmap.org/wiki/Key:surface> .


###  https://w3id.org/openstreetmap/terms#tracktype
:tracktype rdf:type owl:ObjectProperty ;
           rdfs:domain :Way ;
           rdfs:range :TracktypeValue ;
           rdfs:comment "How well-maintained a track is, particularly regarding surface firmness."@en ;
           rdfs:isDefinedBy <https://w3id.org/openstreetmap/terms#> ;
           rdfs:label "tracktype=*"@en ;
           <http://www.w3.org/ns/prov#wasInfluencedBy> <https://wiki.openstreetmap.org/wiki/Key:tracktype> .


###  https://w3id.org/openstreetmap/terms#vehicle
:vehicle rdf:type owl:ObjectProperty ;
         rdfs:domain :Way ;
         rdfs:range :AccessValue ;
         rdfs:comment "The legal access restriction for all types of land-based vehicles not operated upon rails."@en ;
         rdfs:isDefinedBy <https://w3id.org/openstreetmap/terms#> ;
         rdfs:label "vehicle=*"@en ;
         <http://www.w3.org/ns/prov#wasInfluencedBy> <https://wiki.openstreetmap.org/wiki/Key:vehicle> .


#################################################################
#    Data properties
#################################################################

###  http://purl.org/dc/terms/title
<http://purl.org/dc/terms/title> rdf:type owl:DatatypeProperty .


###  https://w3id.org/openstreetmap/terms#hasTag
:hasTag rdf:type owl:DatatypeProperty ;
        rdfs:domain :Element ;
        rdfs:range xsd:string ;
        rdfs:comment """A tag describes the meaning of a particular element in the OSM data model. 
                              It consists of two free format text fields; a 'key' and a 'value' and are formatted as '{key}={value}'. 
                              This property should be used for tags that don't have their semantics explicitly defined. """@en ;
        rdfs:isDefinedBy <https://w3id.org/openstreetmap/terms#> ;
        rdfs:label "hasTag"@en .


###  https://w3id.org/openstreetmap/terms#maxspeed
:maxspeed rdf:type owl:DatatypeProperty ;
          rdfs:domain :Way ;
          rdfs:range xsd:double ;
          <http://qudt.org/schema/qudt/hasUnit> <http://qudt.org/vocab/unit/KM-PER-HR> ;
          rdfs:comment "The maximum legal speed limit, in km/h."@en ;
          rdfs:isDefinedBy <https://w3id.org/openstreetmap/terms#> ;
          rdfs:label "maxspeed=*"@en ;
          <http://www.w3.org/ns/prov#wasInfluencedBy> <https://wiki.openstreetmap.org/wiki/Key:maxspeed> .


###  https://w3id.org/openstreetmap/terms#name
:name rdf:type owl:DatatypeProperty ;
      rdfs:subPropertyOf <http://purl.org/dc/terms/title> ;
      rdfs:domain :Element ;
      rdfs:range rdfs:Literal ;
      rdfs:comment "The default name of an element."@en ;
      rdfs:isDefinedBy <https://w3id.org/openstreetmap/terms#> ;
      rdfs:label "name=*"@en ;
      <http://www.w3.org/ns/prov#wasInfluencedBy> <https://wiki.openstreetmap.org/wiki/Key:name> .


#################################################################
#    Classes
#################################################################

###  http://www.w3.org/1999/02/22-rdf-syntax-ns#list
rdf:list rdf:type owl:Class .


###  http://xmlns.com/foaf/0.1/Document
<http://xmlns.com/foaf/0.1/Document> rdf:type owl:Class .


###  http://xmlns.com/foaf/0.1/Person
<http://xmlns.com/foaf/0.1/Person> rdf:type owl:Class .


###  https://w3id.org/openstreetmap/terms#AccessValue
:AccessValue rdf:type owl:Class ;
             rdfs:comment "The legal access for highways and other transportation networks."@en ;
             rdfs:isDefinedBy <https://w3id.org/openstreetmap/terms#> ;
             rdfs:label "AccessValue"@en ;
             <http://www.w3.org/ns/prov#wasInfluencedBy> <https://wiki.openstreetmap.org/wiki/Key:access> .


###  https://w3id.org/openstreetmap/terms#BarrierValue
:BarrierValue rdf:type owl:Class ;
              rdfs:comment "A physical structure which blocks or impedes movement."@en ;
              rdfs:isDefinedBy <https://w3id.org/openstreetmap/terms#> ;
              rdfs:label "BarrierValue"@en ;
              <http://www.w3.org/ns/prov#wasInfluencedBy> <https://wiki.openstreetmap.org/wiki/Key:barrier> .


###  https://w3id.org/openstreetmap/terms#ConstructionValue
:ConstructionValue rdf:type owl:Class ;
                   rdfs:comment "A feature which is currently under construction."@en ;
                   rdfs:isDefinedBy <https://w3id.org/openstreetmap/terms#> ;
                   rdfs:label "ConstructionValue"@en ;
                   <http://www.w3.org/ns/prov#wasInfluencedBy> <https://wiki.openstreetmap.org/wiki/Key:construction> .


###  https://w3id.org/openstreetmap/terms#CrossingValue
:CrossingValue rdf:type owl:Class ;
               rdfs:comment "A specific type of pedestrian crossing."@en ;
               rdfs:isDefinedBy <https://w3id.org/openstreetmap/terms#> ;
               rdfs:label "CrossingValue"@en ;
               <http://www.w3.org/ns/prov#wasInfluencedBy> <https://wiki.openstreetmap.org/wiki/Key:crossing> .


###  https://w3id.org/openstreetmap/terms#CyclewayValue
:CyclewayValue rdf:type owl:Class ;
               rdfs:comment "Cycling infrastructure that is an inherent part of the road."@en ;
               rdfs:isDefinedBy <https://w3id.org/openstreetmap/terms#> ;
               rdfs:label "CyclewayValue"@en ;
               <http://www.w3.org/ns/prov#wasInfluencedBy> <https://wiki.openstreetmap.org/wiki/Key:cycleway> .


###  https://w3id.org/openstreetmap/terms#Element
:Element rdf:type owl:Class ;
         owl:equivalentClass [ rdf:type owl:Class ;
                               owl:unionOf ( :Node
                                             :Relation
                                             :Way
                                           )
                             ] ;
         rdfs:comment "Elements are the basic components of OpenStreetMap's conceptual data model of the physical world."@en ;
         rdfs:isDefinedBy <https://w3id.org/openstreetmap/terms#> ;
         rdfs:label "Element"@en ;
         <http://www.w3.org/ns/prov#wasInfluencedBy> <https://wiki.openstreetmap.org/wiki/Elements> .


###  https://w3id.org/openstreetmap/terms#FootwayValue
:FootwayValue rdf:type owl:Class ;
              rdfs:comment "A specific kind of footway."@en ;
              rdfs:isDefinedBy <https://w3id.org/openstreetmap/terms#> ;
              rdfs:label "FootwayValue"@en ;
              <http://www.w3.org/ns/prov#wasInfluencedBy> <https://wiki.openstreetmap.org/wiki/Key:footway> .


###  https://w3id.org/openstreetmap/terms#HighwayValue
:HighwayValue rdf:type owl:Class ;
              rdfs:comment "The kind of road, street or path."@en ;
              rdfs:isDefinedBy <https://w3id.org/openstreetmap/terms#> ;
              rdfs:label "HighwayValue"@en ;
              <http://www.w3.org/ns/prov#wasInfluencedBy> <https://wiki.openstreetmap.org/wiki/Key:highway> .


###  https://w3id.org/openstreetmap/terms#Node
:Node rdf:type owl:Class ;
      rdfs:subClassOf <https://www.w3.org/2003/01/geo/wgs84_pos#Point> ;
      owl:disjointWith :Relation ,
                       :Way ;
      rdfs:comment """A node is one of the core elements in the OpenStreetMap data model.
                              It consists of a single point in space defined by its latitude, longitude and node id."""@en ;
      rdfs:isDefinedBy <https://w3id.org/openstreetmap/terms#> ;
      rdfs:label "Node"@en ;
      <http://www.w3.org/ns/prov#wasInfluencedBy> <https://wiki.openstreetmap.org/wiki/Node> .


###  https://w3id.org/openstreetmap/terms#OnewayValue
:OnewayValue rdf:type owl:Class ;
             rdfs:comment "Direction restrictions."@en ;
             rdfs:isDefinedBy <https://w3id.org/openstreetmap/terms#> ;
             rdfs:label "OnewayValue"@en ;
             <http://www.w3.org/ns/prov#wasInfluencedBy> <https://wiki.openstreetmap.org/wiki/Key:oneway> .


###  https://w3id.org/openstreetmap/terms#Relation
:Relation rdf:type owl:Class ;
          owl:disjointWith :Way ;
          rdfs:comment """A relation consists of one or more tags and also an ordered list of one or more nodes, ways and/or relations as members.
                              It is used to define logical or geographic relationships between other elements."""@en ;
          rdfs:isDefinedBy <https://w3id.org/openstreetmap/terms#> ;
          rdfs:label "Relation"@en ;
          <http://www.w3.org/ns/prov#wasInfluencedBy> <https://wiki.openstreetmap.org/wiki/Relation> .


###  https://w3id.org/openstreetmap/terms#SmoothnessValue
:SmoothnessValue rdf:type owl:Class ;
                 rdfs:comment "A classification scheme regarding the physical usability of a way."@en ;
                 rdfs:isDefinedBy <https://w3id.org/openstreetmap/terms#> ;
                 rdfs:label "SmoothnessValue"@en ;
                 <http://www.w3.org/ns/prov#wasInfluencedBy> <https://wiki.openstreetmap.org/wiki/Key:smoothness> .


###  https://w3id.org/openstreetmap/terms#SurfaceValue
:SurfaceValue rdf:type owl:Class ;
              rdfs:comment "The physical surface of elements, particularly regarding material composition and/or structure."@en ;
              rdfs:isDefinedBy <https://w3id.org/openstreetmap/terms#> ;
              rdfs:label "SurfaceValue"@en ;
              <http://www.w3.org/ns/prov#wasInfluencedBy> <https://wiki.openstreetmap.org/wiki/Key:surface> .


###  https://w3id.org/openstreetmap/terms#TracktypeValue
:TracktypeValue rdf:type owl:Class ;
                rdfs:comment "How well-maintained a track is, particularly regarding surface firmness."@en ;
                rdfs:isDefinedBy <https://w3id.org/openstreetmap/terms#> ;
                rdfs:label "TracktypeValue"@en ;
                <http://www.w3.org/ns/prov#wasInfluencedBy> <https://wiki.openstreetmap.org/wiki/Key:tracktype> .


###  https://w3id.org/openstreetmap/terms#Way
:Way rdf:type owl:Class ;
     rdfs:comment "A way is an ordered list of nodes which normally also has at least one tag."@en ;
     rdfs:isDefinedBy <https://w3id.org/openstreetmap/terms#> ;
     rdfs:label "Way"@en ;
     <http://www.w3.org/ns/prov#wasInfluencedBy> <https://wiki.openstreetmap.org/wiki/Way> .


###  https://www.w3.org/2003/01/geo/wgs84_pos#Point
<https://www.w3.org/2003/01/geo/wgs84_pos#Point> rdf:type owl:Class .


#################################################################
#    Individuals
#################################################################

###  http://www.wikidata.org/entity/Q12511
<http://www.wikidata.org/entity/Q12511> rdf:type owl:NamedIndividual ;
                                        owl:sameAs :Steps .


###  http://www.wikidata.org/entity/Q1302778
<http://www.wikidata.org/entity/Q1302778> rdf:type owl:NamedIndividual ;
                                          owl:sameAs :Trunk .


###  http://www.wikidata.org/entity/Q1628979
<http://www.wikidata.org/entity/Q1628979> rdf:type owl:NamedIndividual ;
                                          owl:sameAs :CycleHighway ,
                                                     :LivingStreet .


###  http://www.wikidata.org/entity/Q189259
<http://www.wikidata.org/entity/Q189259> rdf:type owl:NamedIndividual ;
                                         owl:sameAs :Asphalt .


###  http://www.wikidata.org/entity/Q3352369
<http://www.wikidata.org/entity/Q3352369> rdf:type owl:NamedIndividual ;
                                          owl:sameAs :FootHighway .


###  http://www.wikidata.org/entity/Q46622
<http://www.wikidata.org/entity/Q46622> rdf:type owl:NamedIndividual ;
                                        owl:sameAs :Motorway .


###  http://www.wikidata.org/entity/Q8010
<http://www.wikidata.org/entity/Q8010> rdf:type owl:NamedIndividual ;
                                       owl:sameAs :HighwayCrossing .


###  https://biblio.ugent.be/person/802002413821
<https://biblio.ugent.be/person/802002413821> rdf:type owl:NamedIndividual ,
                                                       <http://xmlns.com/foaf/0.1/Person> ;
                                              <http://xmlns.com/foaf/0.1/mbox> "harm.delva@ugent.be" ;
                                              <http://xmlns.com/foaf/0.1/name> "Harm Delva" .


###  https://w3id.org/openstreetmap/terms
<https://w3id.org/openstreetmap/terms> rdf:type owl:NamedIndividual ,
                                                <http://xmlns.com/foaf/0.1/Document> ;
                                       <http://xmlns.com/foaf/0.1/primaryTopic> <https://w3id.org/openstreetmap/terms#> .


###  https://w3id.org/openstreetmap/terms#Agricultural
:Agricultural rdf:type owl:NamedIndividual ,
                       :AccessValue ;
              rdfs:comment "Only for agricultural traffic."@en ;
              rdfs:isDefinedBy <https://w3id.org/openstreetmap/terms#> ;
              rdfs:label "access=agricultural"@en ;
              <http://www.w3.org/ns/prov#wasInfluencedBy> <https://wiki.openstreetmap.org/wiki/Key:access> .


###  https://w3id.org/openstreetmap/terms#Asphalt
:Asphalt rdf:type owl:NamedIndividual ,
                  :SurfaceValue ;
         rdfs:comment "This road has an asphalt surface."@en ;
         rdfs:isDefinedBy <https://w3id.org/openstreetmap/terms#> ;
         rdfs:label "surface=asphalt"@en ;
         <http://www.w3.org/ns/prov#wasInfluencedBy> <https://wiki.openstreetmap.org/wiki/Tag%3Asurface%3Dasphalt> .


###  https://w3id.org/openstreetmap/terms#BadSmoothness
:BadSmoothness rdf:type owl:NamedIndividual ,
                        :SmoothnessValue ;
               rdfs:comment "Usable by trekking bikes, normal cars and everything that can use roads with 'very bad' smoothness."@en ;
               rdfs:isDefinedBy <https://w3id.org/openstreetmap/terms#> ;
               rdfs:label "smoothness=bad"@en ;
               <http://www.w3.org/ns/prov#wasInfluencedBy> <https://wiki.openstreetmap.org/wiki/Key:smoothness> .


###  https://w3id.org/openstreetmap/terms#Bidirectional
:Bidirectional rdf:type owl:NamedIndividual ,
                        :OnewayValue ;
               rdfs:comment "This is not a oneway street."@en ;
               rdfs:isDefinedBy <https://w3id.org/openstreetmap/terms#> ;
               rdfs:label "oneway=no"@en ;
               <http://www.w3.org/ns/prov#wasInfluencedBy> <https://wiki.openstreetmap.org/wiki/Key:oneway> .


###  https://w3id.org/openstreetmap/terms#Block
:Block rdf:type owl:NamedIndividual ,
                :BarrierValue ;
       rdfs:comment "A large, solid, immobile block that can be moved only with heavy machinery or great effort."@en ;
       rdfs:isDefinedBy <https://w3id.org/openstreetmap/terms#> ;
       rdfs:label "barrier=block"@en ;
       <http://www.w3.org/ns/prov#wasInfluencedBy> <https://wiki.openstreetmap.org/wiki/Key:barrier> .


###  https://w3id.org/openstreetmap/terms#Bollard
:Bollard rdf:type owl:NamedIndividual ,
                  :BarrierValue ;
         rdfs:comment "Solid (usually concrete or metal) pillar or pillars in the middle of the road to prevent passage by some traffic."@en ;
         rdfs:isDefinedBy <https://w3id.org/openstreetmap/terms#> ;
         rdfs:label "barrier=bollard"@en ;
         <http://www.w3.org/ns/prov#wasInfluencedBy> <https://wiki.openstreetmap.org/wiki/Key:bollard> .


###  https://w3id.org/openstreetmap/terms#BorderControl
:BorderControl rdf:type owl:NamedIndividual ,
                        :BarrierValue ;
               rdfs:comment "This is a control point at an international border between two countries. Passports or other forms of ID will be checked."@en ;
               rdfs:isDefinedBy <https://w3id.org/openstreetmap/terms#> ;
               rdfs:label "barrier=border_control"@en ;
               <http://www.w3.org/ns/prov#wasInfluencedBy> <https://wiki.openstreetmap.org/wiki/Key:border_control> .


###  https://w3id.org/openstreetmap/terms#Bridleway
:Bridleway rdf:type owl:NamedIndividual ,
                    :HighwayValue ;
           rdfs:comment "A way intended for use by horse riders."@en ;
           rdfs:isDefinedBy <https://w3id.org/openstreetmap/terms#> ;
           rdfs:label "highway=bridleway"@en ;
           <http://www.w3.org/ns/prov#wasInfluencedBy> <https://wiki.openstreetmap.org/wiki/Tag%3Ahighway%3Dbridleway> .


###  https://w3id.org/openstreetmap/terms#BumpGate
:BumpGate rdf:type owl:NamedIndividual ,
                   :BarrierValue ;
          rdfs:comment "A bump gate is a drive-through gate used in rural areas to provide a barrier to livestock that does not require the driver to exit the vehicle."@en ;
          rdfs:isDefinedBy <https://w3id.org/openstreetmap/terms#> ;
          rdfs:label "barrier=bump_gate"@en ;
          <http://www.w3.org/ns/prov#wasInfluencedBy> <https://en.wikipedia.org/wiki/Bump_gate> .


###  https://w3id.org/openstreetmap/terms#BusTrap
:BusTrap rdf:type owl:NamedIndividual ,
                  :BarrierValue ;
         rdfs:comment "A bus trap is a metal grate placed over a ditch or pit in the road with tines (sides) spaced far enough apart that small-diameter-wheeled (narrower axle) vehicles fall in between the tines but close enough that larger-diameter-wheeled vehicles, such as buses, may pass."@en ;
         rdfs:isDefinedBy <https://w3id.org/openstreetmap/terms#> ;
         rdfs:label "barrier=bus_trap"@en ;
         <http://www.w3.org/ns/prov#wasInfluencedBy> <https://en.wikipedia.org/wiki/Bus_trap> .


###  https://w3id.org/openstreetmap/terms#CattleGrid
:CattleGrid rdf:type owl:NamedIndividual ,
                     :BarrierValue ;
            rdfs:comment "Bars in the road surface that allow wheeled vehicles but not animals to cross."@en ;
            rdfs:isDefinedBy <https://w3id.org/openstreetmap/terms#> ;
            rdfs:label "barrier=cattle_grid"@en ;
            <http://www.w3.org/ns/prov#wasInfluencedBy> <https://wiki.openstreetmap.org/wiki/Key:barrier> .


###  https://w3id.org/openstreetmap/terms#Chain
:Chain rdf:type owl:NamedIndividual ,
                :BarrierValue ;
       rdfs:comment "A chain used to prevent motorised vehicles."@en ;
       rdfs:isDefinedBy <https://w3id.org/openstreetmap/terms#> ;
       rdfs:label "barrier=chain"@en ;
       <http://www.w3.org/ns/prov#wasInfluencedBy> <https://wiki.openstreetmap.org/wiki/Key:barrier> .


###  https://w3id.org/openstreetmap/terms#Cobblestone
:Cobblestone rdf:type owl:NamedIndividual ,
                      :SurfaceValue ;
             rdfs:comment "This road has an cobblestone surface."@en ;
             rdfs:isDefinedBy <https://w3id.org/openstreetmap/terms#> ;
             rdfs:label "surface=cobblestone"@en ;
             <http://www.w3.org/ns/prov#wasInfluencedBy> <https://wiki.openstreetmap.org/wiki/Key:surface> .


###  https://w3id.org/openstreetmap/terms#Compacted
:Compacted rdf:type owl:NamedIndividual ,
                    :SurfaceValue ;
           rdfs:comment "A mixture of larger (e.g., gravel) and smaller (e.g., sand) parts, compacted so the surface is more stable than loose gravel."@en ;
           rdfs:isDefinedBy <https://w3id.org/openstreetmap/terms#> ;
           rdfs:label "surface=compacted"@en ;
           <http://www.w3.org/ns/prov#wasInfluencedBy> <https://wiki.openstreetmap.org/wiki/Tag%3Asurface%3Dcompacted> .


###  https://w3id.org/openstreetmap/terms#Concrete
:Concrete rdf:type owl:NamedIndividual ,
                   :SurfaceValue ;
          rdfs:comment "Cement based concrete."@en ;
          rdfs:isDefinedBy <https://w3id.org/openstreetmap/terms#> ;
          rdfs:label "surface=concrete"@en ;
          <http://www.w3.org/ns/prov#wasInfluencedBy> <https://wiki.openstreetmap.org/wiki/Key:surface> .


###  https://w3id.org/openstreetmap/terms#Customers
:Customers rdf:type owl:NamedIndividual ,
                    :AccessValue ;
           rdfs:comment "Only for customers of the element."@en ;
           rdfs:isDefinedBy <https://w3id.org/openstreetmap/terms#> ;
           rdfs:label "access=customers"@en ;
           <http://www.w3.org/ns/prov#wasInfluencedBy> <https://wiki.openstreetmap.org/wiki/Key:access> .


###  https://w3id.org/openstreetmap/terms#CycleBarrier
:CycleBarrier rdf:type owl:NamedIndividual ,
                       :BarrierValue ;
              rdfs:comment "Barriers to bicycle traffic, most typically a pair of staggered steel bars perpendicular to the way itself whose gaps allow pedestrians to pass."@en ;
              rdfs:isDefinedBy <https://w3id.org/openstreetmap/terms#> ;
              rdfs:label "barrier=cycle_barrier"@en ;
              <http://www.w3.org/ns/prov#wasInfluencedBy> <https://wiki.openstreetmap.org/wiki/Key:barrier> .


###  https://w3id.org/openstreetmap/terms#CycleHighway
:CycleHighway rdf:type owl:NamedIndividual ,
                       :HighwayValue ;
              rdfs:comment "For designated cycleways."@en ;
              rdfs:isDefinedBy <https://w3id.org/openstreetmap/terms#> ;
              rdfs:label "highway=cycleway"@en ;
              <http://www.w3.org/ns/prov#wasInfluencedBy> <https://wiki.openstreetmap.org/wiki/Key:highway> .


###  https://w3id.org/openstreetmap/terms#Debris
:Debris rdf:type owl:NamedIndividual ,
                 :BarrierValue ;
        rdfs:comment "A road is blocked by debris with or without ground. This might be for short or long time. Often used as first step in blocking an abandoned road."@en ;
        rdfs:isDefinedBy <https://w3id.org/openstreetmap/terms#> ;
        rdfs:label "barrier=debris"@en ;
        <http://www.w3.org/ns/prov#wasInfluencedBy> <https://wiki.openstreetmap.org/wiki/Key:barrier> .


###  https://w3id.org/openstreetmap/terms#Delivery
:Delivery rdf:type owl:NamedIndividual ,
                   :AccessValue ;
          rdfs:comment "Only when delivering to the element."@en ;
          rdfs:isDefinedBy <https://w3id.org/openstreetmap/terms#> ;
          rdfs:label "access=customers"@en ;
          <http://www.w3.org/ns/prov#wasInfluencedBy> <https://wiki.openstreetmap.org/wiki/Key:access> .


###  https://w3id.org/openstreetmap/terms#Designated
:Designated rdf:type owl:NamedIndividual ,
                     :AccessValue ;
            rdfs:comment "A preferred or designated route."@en ;
            rdfs:isDefinedBy <https://w3id.org/openstreetmap/terms#> ;
            rdfs:label "access=designated"@en ;
            <http://www.w3.org/ns/prov#wasInfluencedBy> <https://wiki.openstreetmap.org/wiki/Key:access> .


###  https://w3id.org/openstreetmap/terms#Destination
:Destination rdf:type owl:NamedIndividual ,
                      :AccessValue ;
             rdfs:comment "Only when travelling to this element/area; i.e., local traffic only."@en ;
             rdfs:isDefinedBy <https://w3id.org/openstreetmap/terms#> ;
             rdfs:label "access=destination"@en ;
             <http://www.w3.org/ns/prov#wasInfluencedBy> <https://wiki.openstreetmap.org/wiki/Key:access> .


###  https://w3id.org/openstreetmap/terms#Dirt
:Dirt rdf:type owl:NamedIndividual ,
               :SurfaceValue ;
      rdfs:comment "This road's surface is just dirt (earth)."@en ;
      rdfs:isDefinedBy <https://w3id.org/openstreetmap/terms#> ;
      rdfs:label "surface=dirt"@en ;
      <http://www.w3.org/ns/prov#wasInfluencedBy> <https://wiki.openstreetmap.org/wiki/Key:surface> .


###  https://w3id.org/openstreetmap/terms#Discouraged
:Discouraged rdf:type owl:NamedIndividual ,
                      :AccessValue ;
             rdfs:comment "A legal right of way exists but usage is officially discouraged."@en ;
             rdfs:isDefinedBy <https://w3id.org/openstreetmap/terms#> ;
             rdfs:label "access=discouraged"@en ;
             <http://www.w3.org/ns/prov#wasInfluencedBy> <https://wiki.openstreetmap.org/wiki/Key:access> .


###  https://w3id.org/openstreetmap/terms#Dismount
:Dismount rdf:type owl:NamedIndividual ,
                   :AccessValue ;
          rdfs:comment "Permitted for some vehicle (or animal) only if you dismount."@en ;
          rdfs:isDefinedBy <https://w3id.org/openstreetmap/terms#> ;
          rdfs:label "access=dismount"@en ;
          <http://www.w3.org/ns/prov#wasInfluencedBy> <https://wiki.openstreetmap.org/wiki/Key:access> .


###  https://w3id.org/openstreetmap/terms#Emergency
:Emergency rdf:type owl:NamedIndividual ,
                    :AccessValue ;
           rdfs:comment "Only for emergency vehicles."@en ;
           rdfs:isDefinedBy <https://w3id.org/openstreetmap/terms#> ;
           rdfs:label "access=emergency"@en .


###  https://w3id.org/openstreetmap/terms#Entrance
:Entrance rdf:type owl:NamedIndividual ,
                   :BarrierValue ;
          rdfs:comment "A gap in a linear barrier with nothing that limits passing through."@en ;
          rdfs:isDefinedBy <https://w3id.org/openstreetmap/terms#> ;
          rdfs:label "barrier=entrance"@en ;
          <http://www.w3.org/ns/prov#wasInfluencedBy> <https://wiki.openstreetmap.org/wiki/Key:barrier> .


###  https://w3id.org/openstreetmap/terms#ExcellentSmoothness
:ExcellentSmoothness rdf:type owl:NamedIndividual ,
                              :SmoothnessValue ;
                     rdfs:comment "Usable by roller blades, skate boards and everything that can use roads with 'good' smoothness."@en ;
                     rdfs:isDefinedBy <https://w3id.org/openstreetmap/terms#> ;
                     rdfs:label "smoothness=excellent"@en ;
                     <http://www.w3.org/ns/prov#wasInfluencedBy> <https://wiki.openstreetmap.org/wiki/Key:smoothness> .


###  https://w3id.org/openstreetmap/terms#FineGravel
:FineGravel rdf:type owl:NamedIndividual ,
                     :SurfaceValue ;
            rdfs:comment "A multilayer pavement with a stone or gravel basis and a topmost surface of firm, granular gravel."@en ;
            rdfs:isDefinedBy <https://w3id.org/openstreetmap/terms#> ;
            rdfs:label "surface=fine_gravel"@en ;
            <http://www.w3.org/ns/prov#wasInfluencedBy> <https://wiki.openstreetmap.org/wiki/Key:surface> .


###  https://w3id.org/openstreetmap/terms#FootHighway
:FootHighway rdf:type owl:NamedIndividual ,
                      :HighwayValue ;
             rdfs:comment "Designated footpaths; i.e., mainly/exclusively for pedestrians."@en ;
             rdfs:isDefinedBy <https://w3id.org/openstreetmap/terms#> ;
             rdfs:label "highway=footway"@en ;
             <http://www.w3.org/ns/prov#wasInfluencedBy> <https://wiki.openstreetmap.org/wiki/Key:highway> .


###  https://w3id.org/openstreetmap/terms#Forestry
:Forestry rdf:type owl:NamedIndividual ,
                   :AccessValue ;
          rdfs:comment "Only for forestry traffic."@en ;
          rdfs:isDefinedBy <https://w3id.org/openstreetmap/terms#> ;
          rdfs:label "access=forestry"@en ;
          <http://www.w3.org/ns/prov#wasInfluencedBy> <https://wiki.openstreetmap.org/wiki/Key:access> .


###  https://w3id.org/openstreetmap/terms#FreeAccess
:FreeAccess rdf:type owl:NamedIndividual ,
                     :AccessValue ;
            rdfs:comment "The public has an official, legally-enshrined right of access; i.e., it's a right of way."@en ;
            rdfs:isDefinedBy <https://w3id.org/openstreetmap/terms#> ;
            rdfs:label "access=yes"@en ;
            <http://www.w3.org/ns/prov#wasInfluencedBy> <https://wiki.openstreetmap.org/wiki/Key:access> .


###  https://w3id.org/openstreetmap/terms#Gate
:Gate rdf:type owl:NamedIndividual ,
               :BarrierValue ;
      rdfs:comment "An entrance that can be opened or closed to get through the barrier."@en ;
      rdfs:isDefinedBy <https://w3id.org/openstreetmap/terms#> ;
      rdfs:label "barrier=gate"@en ;
      <http://www.w3.org/ns/prov#wasInfluencedBy> <https://wiki.openstreetmap.org/wiki/Key:barrier> .


###  https://w3id.org/openstreetmap/terms#GiveWay
:GiveWay rdf:type owl:NamedIndividual ,
                  :HighwayValue ;
         rdfs:comment "Points where a traffic sign instructs traffic to cede priority."@en ;
         rdfs:isDefinedBy <https://w3id.org/openstreetmap/terms#> ;
         rdfs:label "highway=give_way"@en ;
         <http://www.w3.org/ns/prov#wasInfluencedBy> <https://wiki.openstreetmap.org/wiki/Tag%3Ahighway%3Dgive_way> .


###  https://w3id.org/openstreetmap/terms#GoodSmoothness
:GoodSmoothness rdf:type owl:NamedIndividual ,
                         :SmoothnessValue ;
                rdfs:comment "Usable by racing bikes and everything that can use roads with 'intermediate' smoothness."@en ;
                rdfs:isDefinedBy <https://w3id.org/openstreetmap/terms#> ;
                rdfs:label "smoothness=good"@en ;
                <http://www.w3.org/ns/prov#wasInfluencedBy> <https://wiki.openstreetmap.org/wiki/Key:smoothness> .


###  https://w3id.org/openstreetmap/terms#Grade1
:Grade1 rdf:type owl:NamedIndividual ,
                 :TracktypeValue ;
        rdfs:comment "Solid. Usually a paved or sealed surface."@en ;
        rdfs:isDefinedBy <https://w3id.org/openstreetmap/terms#> ;
        rdfs:label "tracktype=grade1"@en ;
        <http://www.w3.org/ns/prov#wasInfluencedBy> <https://wiki.openstreetmap.org/wiki/Key:tracktype> .


###  https://w3id.org/openstreetmap/terms#Grade2
:Grade2 rdf:type owl:NamedIndividual ,
                 :TracktypeValue ;
        rdfs:comment "Solid. Usually an unpaved track with surface of gravel."@en ;
        rdfs:isDefinedBy <https://w3id.org/openstreetmap/terms#> ;
        rdfs:label "tracktype=grade2"@en ;
        <http://www.w3.org/ns/prov#wasInfluencedBy> <https://wiki.openstreetmap.org/wiki/Key:tracktype> .


###  https://w3id.org/openstreetmap/terms#Grade3
:Grade3 rdf:type owl:NamedIndividual ,
                 :TracktypeValue ;
        rdfs:comment "Mostly solid. Even mixture of hard and soft materials."@en ;
        rdfs:isDefinedBy <https://w3id.org/openstreetmap/terms#> ;
        rdfs:label "tracktype=grade3"@en ;
        <http://www.w3.org/ns/prov#wasInfluencedBy> <https://wiki.openstreetmap.org/wiki/Key:tracktype> .


###  https://w3id.org/openstreetmap/terms#Grade4
:Grade4 rdf:type owl:NamedIndividual ,
                 :TracktypeValue ;
        rdfs:comment "Mostly soft. Almost always an unpaved track prominently with soil/sand/grass, but with some hard or compacted materials mixed in."@en ;
        rdfs:isDefinedBy <https://w3id.org/openstreetmap/terms#> ;
        rdfs:label "tracktype=grade4"@en ;
        <http://www.w3.org/ns/prov#wasInfluencedBy> <https://wiki.openstreetmap.org/wiki/Key:tracktype> .


###  https://w3id.org/openstreetmap/terms#Grade5
:Grade5 rdf:type owl:NamedIndividual ,
                 :TracktypeValue ;
        rdfs:comment "Soft. Almost always an unpaved track lacking additional materials, same surface as surrounding terrain."@en ;
        rdfs:isDefinedBy <https://w3id.org/openstreetmap/terms#> ;
        rdfs:label "tracktype=grade5"@en ;
        <http://www.w3.org/ns/prov#wasInfluencedBy> <https://wiki.openstreetmap.org/wiki/Key:tracktype> .


###  https://w3id.org/openstreetmap/terms#Grass
:Grass rdf:type owl:NamedIndividual ,
                :SurfaceValue ;
       rdfs:comment "Grass covered ground."@en ;
       rdfs:isDefinedBy <https://w3id.org/openstreetmap/terms#> ;
       rdfs:label "surface=grass"@en ;
       <http://www.w3.org/ns/prov#wasInfluencedBy> <https://wiki.openstreetmap.org/wiki/Key:surface> .


###  https://w3id.org/openstreetmap/terms#Gravel
:Gravel rdf:type owl:NamedIndividual ,
                 :SurfaceValue ;
        rdfs:comment "Broken/crushed rock with sharp edges."@en ;
        rdfs:isDefinedBy <https://w3id.org/openstreetmap/terms#> ;
        rdfs:label "surface=gravel"@en ;
        <http://www.w3.org/ns/prov#wasInfluencedBy> <https://wiki.openstreetmap.org/wiki/Key:surface> .


###  https://w3id.org/openstreetmap/terms#Ground
:Ground rdf:type owl:NamedIndividual ,
                 :SurfaceValue ;
        rdfs:comment "No special surface, the ground itself has marks of human or animal usage."@en ;
        rdfs:isDefinedBy <https://w3id.org/openstreetmap/terms#> ;
        rdfs:label "surface=ground"@en ;
        <http://www.w3.org/ns/prov#wasInfluencedBy> <https://wiki.openstreetmap.org/wiki/Key:surface> .


###  https://w3id.org/openstreetmap/terms#HighwayCrossing
:HighwayCrossing rdf:type owl:NamedIndividual ,
                          :HighwayValue ;
                 rdfs:comment "Pedestrians can cross a street here."@en ;
                 rdfs:isDefinedBy <https://w3id.org/openstreetmap/terms#> ;
                 rdfs:label "highway=crossing"@en ;
                 <http://www.w3.org/ns/prov#wasInfluencedBy> <https://wiki.openstreetmap.org/wiki/Tag%3Ahighway%3Dcrossing> .


###  https://w3id.org/openstreetmap/terms#HorribleSmoothness
:HorribleSmoothness rdf:type owl:NamedIndividual ,
                             :SmoothnessValue ;
                    rdfs:comment "Usable by heavy-duty off-road vehicles and everything that can use roads with 'very horrible' smoothness."@en ;
                    rdfs:isDefinedBy <https://w3id.org/openstreetmap/terms#> ;
                    rdfs:label "smoothness=horrible"@en ;
                    <http://www.w3.org/ns/prov#wasInfluencedBy> <https://wiki.openstreetmap.org/wiki/Key:smoothness> .


###  https://w3id.org/openstreetmap/terms#ImpassableSmoothness
:ImpassableSmoothness rdf:type owl:NamedIndividual ,
                               :SmoothnessValue ;
                      rdfs:comment "Not usable by wheeled vehicles."@en ;
                      rdfs:isDefinedBy <https://w3id.org/openstreetmap/terms#> ;
                      rdfs:label "smoothness=impassable"@en ;
                      <http://www.w3.org/ns/prov#wasInfluencedBy> <https://wiki.openstreetmap.org/wiki/Key:smoothness> .


###  https://w3id.org/openstreetmap/terms#InOrder
:InOrder rdf:type owl:NamedIndividual ,
                  :OnewayValue ;
         rdfs:comment "This is a oneway street, with the direction being the same order of the way nodes."@en ;
         rdfs:isDefinedBy <https://w3id.org/openstreetmap/terms#> ;
         rdfs:label "oneway=yes"@en ;
         <http://www.w3.org/ns/prov#wasInfluencedBy> <https://wiki.openstreetmap.org/wiki/Key:oneway> .


###  https://w3id.org/openstreetmap/terms#InReverseOrder
:InReverseOrder rdf:type owl:NamedIndividual ,
                         :OnewayValue ;
                rdfs:comment "This is a oneway street, with the direction being the reverse of the order of the way nodes."@en ;
                rdfs:isDefinedBy <https://w3id.org/openstreetmap/terms#> ;
                rdfs:label "oneway=-1"@en ;
                <http://www.w3.org/ns/prov#wasInfluencedBy> <https://wiki.openstreetmap.org/wiki/Key:oneway> .


###  https://w3id.org/openstreetmap/terms#IntermediateSmoothness
:IntermediateSmoothness rdf:type owl:NamedIndividual ,
                                 :SmoothnessValue ;
                        rdfs:comment "Usable by city bikes, sport cars, wheel chairs and everything that can use roads with 'bad' smoothness."@en ;
                        rdfs:isDefinedBy <https://w3id.org/openstreetmap/terms#> ;
                        rdfs:label "smoothness=intermediate"@en ;
                        <http://www.w3.org/ns/prov#wasInfluencedBy> <https://wiki.openstreetmap.org/wiki/Key:smoothness> .


###  https://w3id.org/openstreetmap/terms#Lane
:Lane rdf:type owl:NamedIndividual ,
               :CyclewayValue ;
      rdfs:comment "Two-way streets where there are cycle lanes on both sides of the road."@en ;
      rdfs:isDefinedBy <https://w3id.org/openstreetmap/terms#> ;
      rdfs:label "cycleway=lane"@en ;
      <http://www.w3.org/ns/prov#wasInfluencedBy> <https://wiki.openstreetmap.org/wiki/Tag%3Acycleway%3Dlane> .


###  https://w3id.org/openstreetmap/terms#LiftGate
:LiftGate rdf:type owl:NamedIndividual ,
                   :BarrierValue ;
          rdfs:comment "A lift gate (boom barrier) is a bar, or pole pivoted in such a way as to allow the boom to block vehicular access through a controlled point."@en ;
          rdfs:isDefinedBy <https://w3id.org/openstreetmap/terms#> ;
          rdfs:label "barrier=lift_gate"@en ;
          <http://www.w3.org/ns/prov#wasInfluencedBy> <https://wiki.openstreetmap.org/wiki/Key:barrier> .


###  https://w3id.org/openstreetmap/terms#LivingStreet
:LivingStreet rdf:type owl:NamedIndividual ,
                       :HighwayValue ;
              rdfs:comment "For living streets, which are residential streets where pedestrians have legal priority over cars."@en ;
              rdfs:isDefinedBy <https://w3id.org/openstreetmap/terms#> ;
              rdfs:label "highway=living_street"@en ;
              <http://www.w3.org/ns/prov#wasInfluencedBy> <https://wiki.openstreetmap.org/wiki/Key:highway> .


###  https://w3id.org/openstreetmap/terms#Motorway
:Motorway rdf:type owl:NamedIndividual ,
                   :HighwayValue ;
          rdfs:comment "A restricted access major divided highway, normally with 2 or more running lanes plus emergency hard shoulder."@en ;
          rdfs:isDefinedBy <https://w3id.org/openstreetmap/terms#> ;
          rdfs:label "highway=motorway"@en ;
          <http://www.w3.org/ns/prov#wasInfluencedBy> <https://wiki.openstreetmap.org/wiki/Key:highway> .


###  https://w3id.org/openstreetmap/terms#MotorwayLink
:MotorwayLink rdf:type owl:NamedIndividual ,
                       :HighwayValue ;
              rdfs:comment "The link roads leading to/from a motorway."@en ;
              rdfs:isDefinedBy <https://w3id.org/openstreetmap/terms#> ;
              rdfs:label "highway=motorway_link"@en ;
              <http://www.w3.org/ns/prov#wasInfluencedBy> <https://wiki.openstreetmap.org/wiki/Key:highway> .


###  https://w3id.org/openstreetmap/terms#Mud
:Mud rdf:type owl:NamedIndividual ,
              :SurfaceValue ;
     rdfs:comment "Like the ground surface, but usually wet."@en ;
     rdfs:isDefinedBy <https://w3id.org/openstreetmap/terms#> ;
     rdfs:label "surface=mud"@en ;
     <http://www.w3.org/ns/prov#wasInfluencedBy> <https://wiki.openstreetmap.org/wiki/Key:surface> .


###  https://w3id.org/openstreetmap/terms#NoAccess
:NoAccess rdf:type owl:NamedIndividual ,
                   :AccessValue ;
          rdfs:comment "No access for the general public."@en ;
          rdfs:isDefinedBy <https://w3id.org/openstreetmap/terms#> ;
          rdfs:label "access=no"@en ;
          <http://www.w3.org/ns/prov#wasInfluencedBy> <https://wiki.openstreetmap.org/wiki/Key:access> .


###  https://w3id.org/openstreetmap/terms#OfficialAccess
:OfficialAccess rdf:type owl:NamedIndividual ,
                         :AccessValue ;
                rdfs:comment "A way legally dedicated to specific modes of travel by a law or by the rules of traffic."@en ;
                rdfs:isDefinedBy <https://w3id.org/openstreetmap/terms#> ;
                rdfs:label "access=official"@en ;
                <http://www.w3.org/ns/prov#wasInfluencedBy> <https://wiki.openstreetmap.org/wiki/Tag:access%3Dofficial> .


###  https://w3id.org/openstreetmap/terms#Opposite
:Opposite rdf:type owl:NamedIndividual ,
                   :CyclewayValue ;
          rdfs:comment "Cyclists are permitted to travel in both directions on a road which is one-way for normal traffic."@en ;
          rdfs:isDefinedBy <https://w3id.org/openstreetmap/terms#> ;
          rdfs:label "cycleway=opposite"@en ;
          <http://www.w3.org/ns/prov#wasInfluencedBy> <https://wiki.openstreetmap.org/wiki/Tag%3Acycleway%3Dopposite> .


###  https://w3id.org/openstreetmap/terms#OppositeLane
:OppositeLane rdf:type owl:NamedIndividual ,
                       :CyclewayValue ;
              rdfs:comment "A one-way street that has a cycling lane going in the opposite direction to normal traffic flow."@en ;
              rdfs:isDefinedBy <https://w3id.org/openstreetmap/terms#> ;
              rdfs:label "cycleway=opposite_lane"@en ;
              <http://www.w3.org/ns/prov#wasInfluencedBy> <https://wiki.openstreetmap.org/wiki/Tag%3Acycleway%3Dopposite_lane> .


###  https://w3id.org/openstreetmap/terms#OppositeTrack
:OppositeTrack rdf:type owl:NamedIndividual ,
                        :CyclewayValue ;
               rdfs:comment "A cycle track travelling in the opposite direction to other traffic."@en ;
               rdfs:isDefinedBy <https://w3id.org/openstreetmap/terms#> ;
               rdfs:label "cycleway=opposite_track"@en ;
               <http://www.w3.org/ns/prov#wasInfluencedBy> <https://wiki.openstreetmap.org/wiki/Tag%3Acycleway%3Dopposite_track> .


###  https://w3id.org/openstreetmap/terms#Path
:Path rdf:type owl:NamedIndividual ,
               :HighwayValue ;
      rdfs:comment "A non-specific path."@en ;
      rdfs:isDefinedBy <https://w3id.org/openstreetmap/terms#> ;
      rdfs:label "highway=path"@en ;
      <http://www.w3.org/ns/prov#wasInfluencedBy> <https://wiki.openstreetmap.org/wiki/Key:highway> .


###  https://w3id.org/openstreetmap/terms#Paved
:Paved rdf:type owl:NamedIndividual ,
                :SurfaceValue ;
       rdfs:comment "A non-specific paved surface."@en ;
       rdfs:isDefinedBy <https://w3id.org/openstreetmap/terms#> ;
       rdfs:label "surface=paved"@en ;
       <http://www.w3.org/ns/prov#wasInfluencedBy> <https://wiki.openstreetmap.org/wiki/Key:surface> .


###  https://w3id.org/openstreetmap/terms#PavingStones
:PavingStones rdf:type owl:NamedIndividual ,
                       :SurfaceValue ;
              rdfs:comment "A relatively smooth surface paved with stones."@en ;
              rdfs:isDefinedBy <https://w3id.org/openstreetmap/terms#> ;
              rdfs:label "surface=paving_stones"@en ;
              <http://www.w3.org/ns/prov#wasInfluencedBy> <https://wiki.openstreetmap.org/wiki/Key:surface> .


###  https://w3id.org/openstreetmap/terms#Pebblestone
:Pebblestone rdf:type owl:NamedIndividual ,
                      :SurfaceValue ;
             rdfs:comment "Loosely arranged smooth stones."@en ;
             rdfs:isDefinedBy <https://w3id.org/openstreetmap/terms#> ;
             rdfs:label "surface=pebblestone"@en ;
             <http://www.w3.org/ns/prov#wasInfluencedBy> <https://wiki.openstreetmap.org/wiki/Key:surface> .


###  https://w3id.org/openstreetmap/terms#Permissive
:Permissive rdf:type owl:NamedIndividual ,
                     :AccessValue ;
            rdfs:comment "Open to general traffic until such time as the owner revokes the permission."@en ;
            rdfs:isDefinedBy <https://w3id.org/openstreetmap/terms#> ;
            rdfs:label "access=permissive"@en ;
            <http://www.w3.org/ns/prov#wasInfluencedBy> <https://wiki.openstreetmap.org/wiki/Key:access> .


###  https://w3id.org/openstreetmap/terms#Primary
:Primary rdf:type owl:NamedIndividual ,
                  :HighwayValue ;
         rdfs:comment "The next most important roads in a country's system, after trunks."@en ;
         rdfs:isDefinedBy <https://w3id.org/openstreetmap/terms#> ;
         rdfs:label "highway=primary"@en ;
         <http://www.w3.org/ns/prov#wasInfluencedBy> <https://wiki.openstreetmap.org/wiki/Key:highway> .


###  https://w3id.org/openstreetmap/terms#PrimaryLink
:PrimaryLink rdf:type owl:NamedIndividual ,
                      :HighwayValue ;
             rdfs:comment "The link roads leading to/from a primary road."@en ;
             rdfs:isDefinedBy <https://w3id.org/openstreetmap/terms#> ;
             rdfs:label "highway=primary_link"@en ;
             <http://www.w3.org/ns/prov#wasInfluencedBy> <https://wiki.openstreetmap.org/wiki/Key:highway> .


###  https://w3id.org/openstreetmap/terms#Private
:Private rdf:type owl:NamedIndividual ,
                  :AccessValue ;
         rdfs:comment "Only with individual permission."@en ;
         rdfs:isDefinedBy <https://w3id.org/openstreetmap/terms#> ;
         rdfs:label "access=private"@en ;
         <http://www.w3.org/ns/prov#wasInfluencedBy> <https://wiki.openstreetmap.org/wiki/Key:access> .


###  https://w3id.org/openstreetmap/terms#Proposed
:Proposed rdf:type owl:NamedIndividual ,
                   :HighwayValue ;
          rdfs:comment "For roads that are about to be built, but where any construction work hasn't yet been started."@en ;
          rdfs:isDefinedBy <https://w3id.org/openstreetmap/terms#> ;
          rdfs:label "highway=proposed"@en ;
          <http://www.w3.org/ns/prov#wasInfluencedBy> <https://wiki.openstreetmap.org/wiki/Tag%3Ahighway%3Dproposed> .


###  https://w3id.org/openstreetmap/terms#Residential
:Residential rdf:type owl:NamedIndividual ,
                      :HighwayValue ;
             rdfs:comment "Roads which serve as an access to housing, without function of connecting settlements. Often lined with housing."@en ;
             rdfs:isDefinedBy <https://w3id.org/openstreetmap/terms#> ;
             rdfs:label "highway=residential"@en ;
             <http://www.w3.org/ns/prov#wasInfluencedBy> <https://wiki.openstreetmap.org/wiki/Key:highway> .


###  https://w3id.org/openstreetmap/terms#Road
:Road rdf:type owl:NamedIndividual ,
               :HighwayValue ;
      rdfs:comment "This tag is used for a road with an unknown classification."@en ;
      rdfs:isDefinedBy <https://w3id.org/openstreetmap/terms#> ;
      rdfs:label "highway=road"@en ;
      <http://www.w3.org/ns/prov#wasInfluencedBy> <https://wiki.openstreetmap.org/wiki/Tag%3Ahighway%3Droad> .


###  https://w3id.org/openstreetmap/terms#SallyPort
:SallyPort rdf:type owl:NamedIndividual ,
                    :BarrierValue ;
           rdfs:comment "A sally port is used to pass through thick or city walls, and is a type of covered gate with two doors."@en ;
           rdfs:isDefinedBy <https://w3id.org/openstreetmap/terms#> ;
           rdfs:label "barrier=sally_port"@en ;
           <http://www.w3.org/ns/prov#wasInfluencedBy> <https://wiki.openstreetmap.org/wiki/Key:barrier> .


###  https://w3id.org/openstreetmap/terms#Sand
:Sand rdf:type owl:NamedIndividual ,
               :SurfaceValue ;
      rdfs:comment "Small to very small fractions of rock."@en ;
      rdfs:isDefinedBy <https://w3id.org/openstreetmap/terms#> ;
      rdfs:label "surface=sand"@en ;
      <http://www.w3.org/ns/prov#wasInfluencedBy> <https://wiki.openstreetmap.org/wiki/Key:surface> .


###  https://w3id.org/openstreetmap/terms#Secondary
:Secondary rdf:type owl:NamedIndividual ,
                    :HighwayValue ;
           rdfs:comment "The next most important roads in a country's system, after primary roads."@en ;
           rdfs:isDefinedBy <https://w3id.org/openstreetmap/terms#> ;
           rdfs:label "highway=secondary"@en ;
           <http://www.w3.org/ns/prov#wasInfluencedBy> <https://wiki.openstreetmap.org/wiki/Key:highway> .


###  https://w3id.org/openstreetmap/terms#SecondaryLink
:SecondaryLink rdf:type owl:NamedIndividual ,
                        :HighwayValue ;
               rdfs:comment "The link roads leading to/from a secondary road."@en ;
               rdfs:isDefinedBy <https://w3id.org/openstreetmap/terms#> ;
               rdfs:label "highway=secondary_link"@en ;
               <http://www.w3.org/ns/prov#wasInfluencedBy> <https://wiki.openstreetmap.org/wiki/Key:highway> .


###  https://w3id.org/openstreetmap/terms#Service
:Service rdf:type owl:NamedIndividual ,
                  :HighwayValue ;
         rdfs:comment "For access roads to, or within an industrial estate, camp site, business park, car park etc."@en ;
         rdfs:isDefinedBy <https://w3id.org/openstreetmap/terms#> ;
         rdfs:label "highway=service"@en ;
         <http://www.w3.org/ns/prov#wasInfluencedBy> <https://wiki.openstreetmap.org/wiki/Key:highway> .


###  https://w3id.org/openstreetmap/terms#Sett
:Sett rdf:type owl:NamedIndividual ,
               :SurfaceValue ;
      rdfs:comment "Sett paving, formed from natural stones cut to a regular shape. The stones do not cover the surface completely, unlike paving_stones."@en ;
      rdfs:isDefinedBy <https://w3id.org/openstreetmap/terms#> ;
      rdfs:label "surface=sett"@en ;
      <http://www.w3.org/ns/prov#wasInfluencedBy> <https://wiki.openstreetmap.org/wiki/Key:surface> .


###  https://w3id.org/openstreetmap/terms#ShareBusway
:ShareBusway rdf:type owl:NamedIndividual ,
                      :CyclewayValue ;
             rdfs:comment "A cycle lane taking the form of a bus lane that is also designated for use by cyclists."@en ;
             rdfs:isDefinedBy <https://w3id.org/openstreetmap/terms#> ;
             rdfs:label "cycleway=share_busway"@en ;
             <http://www.w3.org/ns/prov#wasInfluencedBy> <https://wiki.openstreetmap.org/wiki/Tag%3Acycleway%3Dshare_busway> .


###  https://w3id.org/openstreetmap/terms#Shared
:Shared rdf:type owl:NamedIndividual ,
                 :CyclewayValue ;
        rdfs:comment "In general, this indicates that cyclists share space with other traffic on this highway."@en ;
        rdfs:isDefinedBy <https://w3id.org/openstreetmap/terms#> ;
        rdfs:label "cycleway=shared"@en ;
        <http://www.w3.org/ns/prov#wasInfluencedBy> <https://wiki.openstreetmap.org/wiki/Key:cycleway> .


###  https://w3id.org/openstreetmap/terms#SharedLane
:SharedLane rdf:type owl:NamedIndividual ,
                     :CyclewayValue ;
            rdfs:comment "Roads which contain a shared lane marking, or sharrow, to indicate that the travel lane is shared by bicycles and other vehicles."@en ;
            rdfs:isDefinedBy <https://w3id.org/openstreetmap/terms#> ;
            rdfs:label "cycleway=shared_lane"@en ;
            <http://www.w3.org/ns/prov#wasInfluencedBy> <https://wiki.openstreetmap.org/wiki/Proposed_features/shared_lane> .


###  https://w3id.org/openstreetmap/terms#Sidewalk
:Sidewalk rdf:type owl:NamedIndividual ,
                   :FootwayValue ;
          rdfs:comment "A sidewalk that's distinct from the carriageway."@en ;
          rdfs:isDefinedBy <https://w3id.org/openstreetmap/terms#> ;
          rdfs:label "footway=sidewalk"@en ;
          <http://www.w3.org/ns/prov#wasInfluencedBy> <https://wiki.openstreetmap.org/wiki/Tag%3Afootway%3Dsidewalk> .


###  https://w3id.org/openstreetmap/terms#Steps
:Steps rdf:type owl:NamedIndividual ,
                :HighwayValue ;
       rdfs:comment "Flights of steps on footways and paths."@en ;
       rdfs:isDefinedBy <https://w3id.org/openstreetmap/terms#> ;
       rdfs:label "highway=steps"@en ;
       <http://www.w3.org/ns/prov#wasInfluencedBy> <https://wiki.openstreetmap.org/wiki/Tag%3Ahighway%3Dsteps> .


###  https://w3id.org/openstreetmap/terms#Stop
:Stop rdf:type owl:NamedIndividual ,
               :HighwayValue ;
      rdfs:comment "Points at which vehicles are required to stop."@en ;
      rdfs:isDefinedBy <https://w3id.org/openstreetmap/terms#> ;
      rdfs:label "highway=stop"@en ;
      <http://www.w3.org/ns/prov#wasInfluencedBy> <https://wiki.openstreetmap.org/wiki/Tag%3Ahighway%3Dstop> .


###  https://w3id.org/openstreetmap/terms#SwingGate
:SwingGate rdf:type owl:NamedIndividual ,
                    :BarrierValue ;
           rdfs:comment "Similar to a lift gate but rotates sidewards to open."@en ;
           rdfs:isDefinedBy <https://w3id.org/openstreetmap/terms#> ;
           rdfs:label "barrier=swing_gate"@en ;
           <http://www.w3.org/ns/prov#wasInfluencedBy> <https://wiki.openstreetmap.org/wiki/Key:barrier> .


###  https://w3id.org/openstreetmap/terms#Tertiary
:Tertiary rdf:type owl:NamedIndividual ,
                   :HighwayValue ;
          rdfs:comment "The next most important roads in a country's system, after secondary roads."@en ;
          rdfs:isDefinedBy <https://w3id.org/openstreetmap/terms#> ;
          rdfs:label "highway=tertiary"@en ;
          <http://www.w3.org/ns/prov#wasInfluencedBy> <https://wiki.openstreetmap.org/wiki/Key:highway> .


###  https://w3id.org/openstreetmap/terms#TertiaryLink
:TertiaryLink rdf:type owl:NamedIndividual ,
                       :HighwayValue ;
              rdfs:comment "The link roads leading to/from a tertiary road."@en ;
              rdfs:isDefinedBy <https://w3id.org/openstreetmap/terms#> ;
              rdfs:label "highway=tertiary_link"@en ;
              <http://www.w3.org/ns/prov#wasInfluencedBy> <https://wiki.openstreetmap.org/wiki/Key:highway> .


###  https://w3id.org/openstreetmap/terms#TollBooth
:TollBooth rdf:type owl:NamedIndividual ,
                    :BarrierValue ;
           rdfs:comment "A road usage toll or fee is collected here."@en ;
           rdfs:isDefinedBy <https://w3id.org/openstreetmap/terms#> ;
           rdfs:label "barrier=toll_booth"@en ;
           <http://www.w3.org/ns/prov#wasInfluencedBy> <https://wiki.openstreetmap.org/wiki/Key:barrier> .


###  https://w3id.org/openstreetmap/terms#Track
:Track rdf:type owl:NamedIndividual ,
                :HighwayValue ;
       rdfs:comment "Roads for mostly agricultural or forestry uses. If used in the context of a cycleway this means a cycle track running parallel to a road."@en ;
       rdfs:isDefinedBy <https://w3id.org/openstreetmap/terms#> ;
       rdfs:label "highway=track"@en ;
       <http://www.w3.org/ns/prov#wasInfluencedBy> <https://wiki.openstreetmap.org/wiki/Key:highway> .


###  https://w3id.org/openstreetmap/terms#TrafficSignals
:TrafficSignals rdf:type owl:NamedIndividual ,
                         :HighwayValue ;
                rdfs:comment "Signalling devices positioned at road intersections, pedestrian crossings and other locations to control competing flows of traffic. "@en ;
                rdfs:isDefinedBy <https://w3id.org/openstreetmap/terms#> ;
                rdfs:label "highway=traffic_signals"@en ;
                <http://www.w3.org/ns/prov#wasInfluencedBy> <https://wiki.openstreetmap.org/wiki/Tag%3Ahighway%3Dtraffic_signals> .


###  https://w3id.org/openstreetmap/terms#Trunk
:Trunk rdf:type owl:NamedIndividual ,
                :HighwayValue ;
       rdfs:comment "The most important roads in a country's system that aren't motorways."@en ;
       rdfs:isDefinedBy <https://w3id.org/openstreetmap/terms#> ;
       rdfs:label "highway=trunk"@en ;
       <http://www.w3.org/ns/prov#wasInfluencedBy> <https://wiki.openstreetmap.org/wiki/Key:highway> .


###  https://w3id.org/openstreetmap/terms#TrunkLink
:TrunkLink rdf:type owl:NamedIndividual ,
                    :HighwayValue ;
           rdfs:comment "The link roads leading to/from a trunk road."@en ;
           rdfs:isDefinedBy <https://w3id.org/openstreetmap/terms#> ;
           rdfs:label "highway=trunk_link"@en ;
           <http://www.w3.org/ns/prov#wasInfluencedBy> <https://wiki.openstreetmap.org/wiki/Key:highway> .


###  https://w3id.org/openstreetmap/terms#Turnstile
:Turnstile rdf:type owl:NamedIndividual ,
                    :BarrierValue ;
           rdfs:comment "A turnstile (also called baffle gate) is used to allow one person at a time to pass."@en ;
           rdfs:isDefinedBy <https://w3id.org/openstreetmap/terms#> ;
           rdfs:label "barrier=turnstile"@en ;
           <http://www.w3.org/ns/prov#wasInfluencedBy> <https://wiki.openstreetmap.org/wiki/Key:barrier> .


###  https://w3id.org/openstreetmap/terms#Unclassified
:Unclassified rdf:type owl:NamedIndividual ,
                       :HighwayValue ;
              rdfs:comment "The least important through roads in a country's system."@en ;
              rdfs:isDefinedBy <https://w3id.org/openstreetmap/terms#> ;
              rdfs:label "highway=unclassified"@en ;
              <http://www.w3.org/ns/prov#wasInfluencedBy> <https://wiki.openstreetmap.org/wiki/Key:highway> .


###  https://w3id.org/openstreetmap/terms#Uncontrolled
:Uncontrolled rdf:type owl:NamedIndividual ,
                       :CrossingValue ;
              rdfs:comment "A generic crossing with no traffic-signals of any type, just road markings."@en ;
              rdfs:isDefinedBy <https://w3id.org/openstreetmap/terms#> ;
              rdfs:label "crossing=uncontrolled"@en ;
              <http://www.w3.org/ns/prov#wasInfluencedBy> <https://wiki.openstreetmap.org/wiki/Key:crossing> .


###  https://w3id.org/openstreetmap/terms#UnderConstruction
:UnderConstruction rdf:type owl:NamedIndividual ,
                            :ConstructionValue ;
                   rdfs:comment "Indicates that this element is under construction."@en ;
                   rdfs:isDefinedBy <https://w3id.org/openstreetmap/terms#> ;
                   rdfs:label "construction=yes"@en ;
                   <http://www.w3.org/ns/prov#wasInfluencedBy> <https://wiki.openstreetmap.org/wiki/Tag%3Aconstruction%3Dyes> .


###  https://w3id.org/openstreetmap/terms#UnhewnCobblestone
:UnhewnCobblestone rdf:type owl:NamedIndividual ,
                            :SurfaceValue ;
                   rdfs:comment "Cobblestone paving, formed from natural, uncut, overall rounded stones. Firmly attached to a ground, unlike pebblestone."@en ;
                   rdfs:isDefinedBy <https://w3id.org/openstreetmap/terms#> ;
                   rdfs:label "surface=unhewn_cobblestone"@en ;
                   <http://www.w3.org/ns/prov#wasInfluencedBy> <https://wiki.openstreetmap.org/wiki/Key:surface> .


###  https://w3id.org/openstreetmap/terms#Unmarked
:Unmarked rdf:type owl:NamedIndividual ,
                   :CrossingValue ;
          rdfs:comment "A crossing without road markings or traffic lights"@en ;
          rdfs:isDefinedBy <https://w3id.org/openstreetmap/terms#> ;
          rdfs:label "crossing=unmarked"@en ;
          <http://www.w3.org/ns/prov#wasInfluencedBy> <https://wiki.openstreetmap.org/wiki/Key:crossing> .


###  https://w3id.org/openstreetmap/terms#Unpaved
:Unpaved rdf:type owl:NamedIndividual ,
                  :SurfaceValue ;
         rdfs:comment "A loose covering ranging from compacted stone chippings to earth."@en ;
         rdfs:isDefinedBy <https://w3id.org/openstreetmap/terms#> ;
         rdfs:label "surface=unpaved"@en ;
         <http://www.w3.org/ns/prov#wasInfluencedBy> <https://wiki.openstreetmap.org/wiki/Key:surface> .


###  https://w3id.org/openstreetmap/terms#UseSidepath
:UseSidepath rdf:type owl:NamedIndividual ,
                      :AccessValue ;
             rdfs:comment "Can only be used in countries with compulsory cycleways and gives access information on parallel roads."@en ;
             rdfs:isDefinedBy <https://w3id.org/openstreetmap/terms#> ;
             rdfs:label "access=use_sidepath"@en ;
             <http://www.w3.org/ns/prov#wasInfluencedBy> <https://wiki.openstreetmap.org/wiki/Key:access> .


###  https://w3id.org/openstreetmap/terms#VeryBadSmoothness
:VeryBadSmoothness rdf:type owl:NamedIndividual ,
                            :SmoothnessValue ;
                   rdfs:comment "Usable by cars with high clearance, light-duty off-road vehicles and everything that can use roads with 'horrible' smoothness."@en ;
                   rdfs:isDefinedBy <https://w3id.org/openstreetmap/terms#> ;
                   rdfs:label "smoothness=very_bad"@en ;
                   <http://www.w3.org/ns/prov#wasInfluencedBy> <https://wiki.openstreetmap.org/wiki/Key:smoothness> .


###  https://w3id.org/openstreetmap/terms#VeryHorribleSmoothness
:VeryHorribleSmoothness rdf:type owl:NamedIndividual ,
                                 :SmoothnessValue ;
                        rdfs:comment "Usable by tractors, ATVs and tanks."@en ;
                        rdfs:isDefinedBy <https://w3id.org/openstreetmap/terms#> ;
                        rdfs:label "smoothness=very_horrible"@en ;
                        <http://www.w3.org/ns/prov#wasInfluencedBy> <https://wiki.openstreetmap.org/wiki/Key:smoothness> .


###  https://w3id.org/openstreetmap/terms#Wood
:Wood rdf:type owl:NamedIndividual ,
               :SurfaceValue ;
      rdfs:comment "Wood."@en ;
      rdfs:isDefinedBy <https://w3id.org/openstreetmap/terms#> ;
      rdfs:label "surface=wood"@en ;
      <http://www.w3.org/ns/prov#wasInfluencedBy> <https://wiki.openstreetmap.org/wiki/Key:surface> .


###  Generated by the OWL API (version 5.1.7) https://github.com/owlcs/owlapi/
